LFSemantics.v
@@ -1,6 +1,6 @@
 Require Import LFSubstitution.
 Require Import Setoid.
-
+Require Import LibList.
 Require Import PermutLib.
 Require Import PPermutLib.
 Require Import OkLib.
@@ -62,11 +62,11 @@ Inductive types_LF: Background_LF -> Context_LF -> te_LF -> ty -> Prop :=
   (HT: G |= (w, Gamma) |- M ::: A),
   G |= (w, Gamma) |- get_here_LF (fwo w) M ::: <*> A
 
-| t_get_here_LF: forall A G w Gamma Ctx' M
-  (Ok_Bg: ok_Bg ((w, Gamma) :: G & Ctx'))
-  (HT: G & Ctx' |= (w, Gamma) |- M ::: A),
+| t_get_here_LF: forall A G w Gamma w' Gamma' M
+  (Ok_Bg: ok_Bg ((w, Gamma) :: G & (w', Gamma')))
+  (HT: G & (w', Gamma') |= (w, Gamma) |- M ::: A),
   forall G', (G & (w, Gamma)) ~=~ G' ->
-    G' |= Ctx' |- get_here_LF (fwo w) M ::: <*> A
+    G' |= (w', Gamma') |- get_here_LF (fwo w) M ::: <*> A
 
 | t_letdia_LF: forall L_w L_t A B G w Gamma M N
   (Ok_Bg: ok_Bg ((w, Gamma) :: G))
@@ -107,17 +107,23 @@ Global Reserved Notation " M |-> N " (at level 70).
 *)
 Inductive step_LF: (te_LF * vwo) -> (te_LF * vwo) -> Prop :=
 | red_appl_lam_LF: forall ctx M A N,
-  lc_w_LF M -> (* lc_t_LF M -> *)
+  lc_w_LF M ->
+  (* lc_t_n_LF 1 M -> or (forall x, x \notin L -> lc_t_LF (M ^t^ (fte x))) -> *)
   lc_w_LF N -> lc_t_LF N ->
   (appl_LF (lam_LF A M) N, ctx) |-> ( M ^t^ N , ctx)
 
 | red_unbox_fetch_box_LF: forall ctx ctx' M,
-  (* lc_w_LF M -> *) lc_t_LF M ->
+   (* lc_w_n_LF 1 M -> or
+     (forall x, x \notin L -> lc_w_LF (M ^w^ (fwo x))) -> *)
+  lc_t_LF M ->
   (unbox_fetch_LF ctx' (box_LF M), ctx) |-> (M ^w^ ctx, ctx)
 
 | red_letdia_get_get_here_LF: forall ctx ctx' ctx'' M N,
   lc_w_LF M -> lc_t_LF M ->
-  (* lc_w_LF N -> lc_t_LF N -> *)
+  (* lc_w_n_LF 1 N -> or
+     (forall x, x \notin L_w -> lc_w_LF (N ^w^ (fwo x))) -> *)
+  (* lc_t_n_LF 1 N -> or
+     (forall x, x \notin L_t -> lc_t_LF (N ^t^ (fte x))) -> *)
   (letdia_get_LF ctx' (get_here_LF ctx'' M) N, ctx) |->
     ((N ^w^ ctx'') ^t^ M, ctx)
 
@@ -140,7 +146,10 @@ Inductive step_LF: (te_LF * vwo) -> (te_LF * vwo) -> Prop :=
 | red_letdia_get_LF: forall ctx ctx' M N M'
   (HT: (M, ctx) |-> (M', ctx)),
   lc_w_LF M -> lc_t_LF M ->
-  (* lc_w_LF N -> lc_t_LF N -> *)
+  (* lc_w_n_LF 1 N -> or
+     (forall x, x \notin L_w -> lc_w_LF (N ^w^ (fwo x))) -> *)
+  (* lc_t_n_LF 1 N -> or
+     (forall x, x \notin L_t -> lc_t_LF (N ^t^ (fte x))) -> *)
   (letdia_get_LF ctx M N, ctx') |-> (letdia_get_LF ctx M' N, ctx')
 
 where " M |-> N " := (step_LF M N ) : label_free_is5_scope.
@@ -158,7 +167,6 @@ where " M |-> N " := (step_LF M N ) : label_free_is5_scope.
      * Specific element of background
      * Main context
 *)
-
 
 (* Proof: simple induction on typing rules *)
 Lemma BackgroundSubsetImpl:
@@ -181,8 +189,8 @@ econstructor; auto.
 destruct HSubst as [GT];
 apply t_box_LF with (L:=L \u used_w_vars (G' & (w, Gamma))); intros;
 [ apply ok_Bg_cons_last |
-  apply H; [ | exists GT | ] ]; auto;
-apply ok_Bg_fresh_wo;
+  apply H; [ | exists GT | ] ]; auto; try PPermut_simpl;
+eapply ok_Bg_fresh_wo;
 [ apply ok_Bg_cons_last |
   rewrite notin_union in H1; destruct H1]; auto.
 (* unbox *)
@@ -192,23 +200,21 @@ destruct HSubst as [GT];
 apply t_unbox_fetch_LF with (Gamma:=Gamma) (G:=G++GT).
 apply ok_Bg_ppermut with (G:=(w', Gamma')::G'0);
   [rewrite <- H0; rewrite <- H; rew_app | ]; auto.
-apply IHHT; [exists GT | ]; auto;
-  apply ok_Bg_ppermut with (G:=(w', Gamma')::G'0); auto;
-  rewrite <- H0; rewrite <- H; rew_app; auto.
-transitivity (G' ++ GT); auto;
-transitivity (G & (w, Gamma) ++ GT); [symmetry | ]; auto.
+apply IHHT; [exists GT | ]; auto; try PPermut_simpl.
+apply ok_Bg_ppermut with (G:=(w', Gamma')::G'0); auto.
+rewrite <- H0; rewrite <- H; rew_app; auto.
+transitivity (G' ++ GT); PPermut_simpl; auto.
 (* here *)
 constructor; auto.
 (* get_here *)
 destruct HSubst as [GT];
 apply t_get_here_LF with (Gamma:=Gamma) (G:=G++GT).
-apply ok_Bg_ppermut with (G:=Ctx'::G'0);
+apply ok_Bg_ppermut with (G:=(w', Gamma')::G'0);
   [rewrite <- H0; rewrite <- H; rew_app | ]; auto.
-apply IHHT; [exists GT | ]; auto;
-  apply ok_Bg_ppermut with (G:=Ctx'::G'0); auto;
+apply IHHT; [exists GT | ]; auto; try PPermut_simpl;
+  apply ok_Bg_ppermut with (G:=(w', Gamma')::G'0); auto;
   rewrite <- H0; rewrite <- H; rew_app; auto.
-transitivity (G' ++ GT); auto;
-transitivity (G & (w, Gamma) ++ GT); [symmetry | ]; auto.
+rewrite <- H0; rewrite <- H; rew_app; auto.
 (* letdia *)
 apply t_letdia_LF with (A:=A) (L_t:=L_t)
   (L_w:=L_w \u used_w_vars ((w, Gamma)::G'));
@@ -225,7 +231,7 @@ apply t_letdia_get_LF with (A:=A) (Gamma:=Gamma) (G:=G++GT)
 apply ok_Bg_ppermut with (G:=Ctx' :: G');
   [rewrite <- H1; rewrite <- H0; rew_app | ]; auto.
 apply IHHT.
-  exists GT; auto.
+  exists GT; rew_app; auto.
   apply ok_Bg_ppermut with (G:=Ctx' :: G');
   [ rewrite <- H1; rewrite <- H0; rew_app | ]; auto.
   intros; apply H; auto.
@@ -233,7 +239,7 @@ apply IHHT.
   apply ok_Bg_ppermut with (G:=(w', (v', A) :: nil) :: Ctx' :: G'); auto;
   rewrite <- H1; rewrite <- H0;
   assert ((G & (w, Gamma) ++ GT)  ~=~ (G ++ GT) & (w, Gamma))
-    by (symmetry; auto);
+    by (symmetry; rew_app; auto);
   rewrite H4; destruct Ctx'; auto.
 rewrite <- H1; rewrite <- H0; rew_app; auto.
 Qed.
@@ -304,7 +310,7 @@ econstructor; [ eapply ok_Bg_permut | ]; eauto.
 (* get_here *)
 apply t_get_here_LF with (G:=G) (Gamma:=Gamma); auto.
 apply ok_Bg_ppermut with (G:=(w0, Gamma) :: G & (w, Gamma0)); auto.
-assert (G & (w, Gamma') ~=~ (G & (w, Gamma0))) as H1 by auto;
+assert (G & (w, Gamma'0) ~=~ (G & (w, Gamma0))) as H1 by auto;
 rewrite H1; auto.
 (* letdia *)
 econstructor; [ eapply ok_Bg_permut | | ]; eauto.
@@ -375,20 +381,20 @@ apply t_box_LF with
   (L:=L \u used_w_vars (G' & (w0, Gamma0) & (w', Delta ++ Delta')));
 intros;
 assert (G' & (w', Delta ++ Delta') & (w0, Gamma0) ~=~
-        G' & (w0, Gamma0) & (w', Delta ++ Delta')) by auto;
+        G' & (w0, Gamma0) & (w', Delta ++ Delta')) by (rew_app; auto);
 [ apply ok_Bg_ppermut with (G:=(w0, Gamma0) :: G' & (w', Delta ++ Delta')) |
-  rewrite H3]; auto;
+  rewrite H3]; auto; try PPermut_simpl;
 apply H with (w:=w'0) (Gamma:=nil);
-[ | | rewrite H0 | rewrite H0 in Ok_Bg]; auto;
+[ | | rewrite H0 | rewrite H0 in Ok_Bg]; auto; try PPermut_simpl.
 apply ok_Bg_fresh_wo; auto;
 apply ok_Bg_ppermut with
   (G:=((w0, Gamma0) :: G' & (w', Delta ++ Delta')));
 auto.
 apply t_box_LF with (L:=L \u used_w_vars (G & (w0, Gamma0++Gamma')));
 [ apply ok_Bg_ppermut with (G:= (w0, Gamma0++Gamma') :: G) |
-  intros; eapply H]; auto;
+  intros; eapply H]; auto; try PPermut_simpl;
 apply ok_Bg_fresh_wo; auto;
-apply ok_Bg_ppermut with (G:=(w0, Gamma0++Gamma')::G); auto.
+apply ok_Bg_ppermut with (G:=(w0, Gamma0++Gamma')::G); auto; PPermut_simpl.
 (* unbox *)
 constructor; [ | eapply IHHT]; eauto.
 constructor; [ | eapply IHHT]; eauto.
@@ -406,41 +412,41 @@ assert ((w0, Gamma0) :: G'0 & (w, Delta ++ Delta') ~=~
   (rewrite H3;
    transitivity ((w, Delta ++ Delta') :: G'0 & (w0, Gamma0));
      [ transitivity ((w0, Gamma0) :: (w, Delta ++ Delta') :: G'0) | ]; auto;
-       transitivity ((w, Delta ++ Delta') :: (w0, Gamma0) :: G'0); auto);
+       transitivity ((w, Delta ++ Delta') :: (w0, Gamma0) :: G'0);
+       auto; PPermut_simpl);
 apply t_unbox_fetch_LF with (G:=G) (Gamma:=Gamma++Delta');
 [rewrite <- H4 | apply IHHT | rewrite H3]; auto; rewrite <- H4; auto.
 (* <> *)
-assert (exists G0, exists G1, G'0 = G0 & (w, Gamma) ++ G1) as H2 by
+assert (exists Gamma', exists G0, exists G1,
+  Gamma' *=* Gamma /\ G'0 = G0 & (w, Gamma') ++ G1) as H2 by
   ( apply PPermut_split_neq with (G':=G) (w:=w'0) (Gamma := Delta);
     [ symmetry; transitivity G' | ]; auto);
-destruct H2 as [GH]; destruct H2 as [GT]; subst G'0;
+destruct H2 as (Gamma', (GH, (GT, (H2a, H2b)))); subst;
 apply t_unbox_fetch_LF with
   (Gamma:=Gamma) (G:=GH ++ GT & (w'0, Delta ++ Delta')).
 apply ok_Bg_ppermut with
-  (G := (w0, Gamma0) :: (GH & (w, Gamma) ++ GT) & (w'0, Delta ++ Delta')); auto;
-rew_app;
-assert ( GH ++ (w, Gamma) :: GT & (w'0, Delta ++ Delta') ~=~
-       (w, Gamma) :: GH ++ GT ++ (w'0, Delta ++ Delta') :: nil) by auto;
-rewrite H2;
-transitivity (((w, Gamma) :: GH ++ GT ++ (w'0, Delta ++ Delta') :: nil) &
-  (w0, Gamma0)); [ | rew_app]; auto.
+  (G := (w0, Gamma0) :: (GH & (w, Gamma) ++ GT) & (w'0, Delta ++ Delta')); auto.
+rew_app; PPermut_simpl.
+assert ((w0, Gamma0) :: (GH & (w, Gamma) ++ GT) & (w'0, Delta ++ Delta') ~=~
+       ((w0, Gamma0) :: (GH & (w, Gamma') ++ GT) & (w'0, Delta ++ Delta')))
+  by PPermut_simpl.
+rewrite H2; auto.
 apply PPermut_bg with (G:= (GH ++ GT & (w0, Gamma0)) & (w'0, Delta ++ Delta')).
- apply IHHT with (w1:=w) (Gamma1:=Gamma) (G':=GH ++ GT & (w0, Gamma0));
- assert (G ~=~ GH ++ GT & (w'0, Delta)) by
-   ( apply PPermut_last_rev_simpl with (a:=(w, Gamma)); transitivity G';
-     [ | rew_app in *; transitivity (GH ++ (w, Gamma) :: GT & (w'0, Delta))];
-     auto);
- [ |
-   rewrite H2; rew_app |
-   apply ok_Bg_ppermut with (G:= (w0, Gamma0) :: GH ++ (w, Gamma) :: GT &
-     (w'0, Delta ++ Delta'))]; rew_app in *; auto;
-  transitivity (((w0, Gamma0) :: GH ++ GT ++ (w, Gamma) :: nil) &
-    (w'0, Delta++Delta')); [rew_app | ]; auto;
-  transitivity (((w, Gamma) :: GH ++ GT ++ (w0, Gamma0) :: nil) &
-    (w'0, Delta ++ Delta')); [ | rew_app]; auto.
-  rew_app; auto.
-rew_app; transitivity (GH ++ GT ++ (w, Gamma) :: (w'0, Delta++Delta') :: nil);
-[ | symmetry]; auto.
+  apply IHHT with (w1:=w) (Gamma1:=Gamma) (G':=GH ++ GT & (w0, Gamma0));
+  assert (G ~=~ GH ++ GT & (w'0, Delta)) by
+  ( apply PPermut_last_rev_simpl with (a:=(w, Gamma)); auto; transitivity G';
+     [ | rewrite H0]; auto; PPermut_simpl);
+  auto; try PPermut_simpl.
+  apply ok_Bg_ppermut with (G:= (w0, Gamma0) :: GH ++ (w, Gamma) :: GT &
+     (w'0, Delta ++ Delta')); auto; try PPermut_simpl.
+  assert ((w0, Gamma0) :: GH ++ (w, Gamma) :: GT & (w'0, Delta ++ Delta') ~=~
+       ((w0, Gamma0) :: (GH & (w, Gamma') ++ GT) & (w'0, Delta ++ Delta')))
+  by PPermut_simpl.
+  rewrite H3; auto.
+  transitivity (((w0, Gamma0) :: GH ++ GT) &
+    (w'0, Delta++Delta')); [rew_app | ]; auto; PPermut_simpl.
+  transitivity (((w, Gamma) :: GH ++ GT ) &
+    (w'0, Delta ++ Delta')); [ | rew_app]; auto; PPermut_simpl.
 (* unbox_fetch 2 *)
 apply t_unbox_fetch_LF with (G:=G) (Gamma:=Gamma);
 rewrite <- H in H0; [ | apply IHHT with (w1:=w) (Gamma1:=Gamma) |]; auto.
@@ -448,7 +454,7 @@ rewrite <- H in H0; [ | apply IHHT with (w1:=w) (Gamma1:=Gamma) |]; auto.
 constructor; [ | apply IHHT with (w:=w0)(Gamma:=Gamma0)]; auto.
 constructor; [ | apply IHHT]; auto.
 (* get_here 1 *)
-destruct (permut_context_LF_dec (w', Delta) (w, Gamma)) as [Eq|Neq];
+destruct (permut_context_LF_dec (w'0, Delta) (w, Gamma)) as [Eq|Neq];
 simpl in *.
 (* = *)
 destruct Eq; subst;
@@ -461,41 +467,41 @@ assert ((w0, Gamma0) :: G'0 & (w, Delta ++ Delta') ~=~
   (rewrite H3;
    transitivity ((w, Delta ++ Delta') :: G'0 & (w0, Gamma0));
      [ transitivity ((w0, Gamma0) :: (w, Delta ++ Delta') :: G'0) | ]; auto;
-       transitivity ((w, Delta ++ Delta') :: (w0, Gamma0) :: G'0); auto);
+       transitivity ((w, Delta ++ Delta') :: (w0, Gamma0) :: G'0);
+       auto; PPermut_simpl);
 apply t_get_here_LF with (G:=G) (Gamma:=Gamma++Delta');
 [rewrite <- H4 | apply IHHT | rewrite H3]; auto; rewrite <- H4; auto.
 (* <> *)
-assert (exists G0, exists G1, G'0 = G0 & (w, Gamma) ++ G1) as H2 by
-  ( apply PPermut_split_neq with (G':=G) (w:=w') (Gamma := Delta);
+assert (exists Gamma', exists G0, exists G1,
+  Gamma' *=* Gamma /\ G'0 = G0 & (w, Gamma') ++ G1) as H2 by
+  ( apply PPermut_split_neq with (G':=G) (w:=w'0) (Gamma := Delta);
     [ symmetry; transitivity G' | ]; auto);
-destruct H2 as [GH]; destruct H2 as [GT]; subst G'0;
+destruct H2 as (Gamma', (GH, (GT, (H2a, H2b)))); subst;
 apply t_get_here_LF with
-  (Gamma:=Gamma) (G:=GH ++ GT & (w', Delta ++ Delta')).
+  (Gamma:=Gamma) (G:=GH ++ GT & (w'0, Delta ++ Delta')).
 apply ok_Bg_ppermut with
-  (G := (w0, Gamma0) :: (GH & (w, Gamma) ++ GT) & (w', Delta ++ Delta')); auto;
-rew_app;
-assert ( GH ++ (w, Gamma) :: GT & (w', Delta ++ Delta') ~=~
-       (w, Gamma) :: GH ++ GT ++ (w', Delta ++ Delta') :: nil) by auto;
-rewrite H2;
-transitivity (((w, Gamma) :: GH ++ GT ++ (w', Delta ++ Delta') :: nil) &
-  (w0, Gamma0)); [ | rew_app]; auto.
-apply PPermut_bg with (G:= (GH ++ GT & (w0, Gamma0)) & (w', Delta ++ Delta')).
- apply IHHT with (w1:=w) (Gamma1:=Gamma) (G':=GH ++ GT & (w0, Gamma0));
- assert (G ~=~ GH ++ GT & (w', Delta)) by
-   ( apply PPermut_last_rev_simpl with (a:=(w, Gamma)); transitivity G';
-     [ | rew_app in *; transitivity (GH ++ (w, Gamma) :: GT & (w', Delta))];
-     auto);
- [ |
-   rewrite H2; rew_app |
-   apply ok_Bg_ppermut with (G:= (w0, Gamma0) :: GH ++ (w, Gamma) :: GT &
-     (w', Delta ++ Delta'))]; rew_app in *; auto;
-  transitivity (((w0, Gamma0) :: GH ++ GT ++ (w, Gamma) :: nil) &
-    (w', Delta++Delta')); [rew_app | ]; auto;
-  transitivity (((w, Gamma) :: GH ++ GT ++ (w0, Gamma0) :: nil) &
-    (w', Delta ++ Delta')); [ | rew_app]; auto.
-  rew_app; auto.
-rew_app; transitivity (GH ++ GT ++ (w, Gamma) :: (w', Delta++Delta') :: nil);
-[ | symmetry]; auto.
+  (G := (w0, Gamma0) :: (GH & (w, Gamma) ++ GT) & (w'0, Delta ++ Delta')); auto.
+rew_app; PPermut_simpl.
+assert ((w0, Gamma0) :: (GH & (w, Gamma) ++ GT) & (w'0, Delta ++ Delta') ~=~
+       ((w0, Gamma0) :: (GH & (w, Gamma') ++ GT) & (w'0, Delta ++ Delta')))
+  by PPermut_simpl.
+rewrite H2; auto.
+apply PPermut_bg with (G:= (GH ++ GT & (w0, Gamma0)) & (w'0, Delta ++ Delta')).
+  apply IHHT with (w1:=w) (Gamma1:=Gamma) (G':=GH ++ GT & (w0, Gamma0));
+  assert (G ~=~ GH ++ GT & (w'0, Delta)) by
+  ( apply PPermut_last_rev_simpl with (a:=(w, Gamma)); auto; transitivity G';
+     [ | rewrite H0]; auto; PPermut_simpl);
+  auto; try PPermut_simpl.
+  apply ok_Bg_ppermut with (G:= (w0, Gamma0) :: GH ++ (w, Gamma) :: GT &
+     (w'0, Delta ++ Delta')); auto; try PPermut_simpl.
+  assert ((w0, Gamma0) :: GH ++ (w, Gamma) :: GT & (w'0, Delta ++ Delta') ~=~
+       ((w0, Gamma0) :: (GH & (w, Gamma') ++ GT) & (w'0, Delta ++ Delta')))
+  by PPermut_simpl.
+  rewrite H3; auto.
+  transitivity (((w0, Gamma0) :: GH ++ GT) &
+    (w'0, Delta++Delta')); [rew_app | ]; auto; PPermut_simpl.
+  transitivity (((w, Gamma) :: GH ++ GT ) &
+    (w'0, Delta ++ Delta')); [ | rew_app]; auto; PPermut_simpl.
 (* get_here 2 *)
 apply t_get_here_LF with (G:=G) (Gamma:=Gamma);
 rewrite <- H in H0; [ | apply IHHT with (w1:=w) (Gamma1:=Gamma) |]; auto.
@@ -551,15 +557,17 @@ apply ok_Bg_fresh_wo_te;
 auto.
 rewrite <- H4; auto.
 (* <> *)
-assert (exists G0, exists G1, G' = G0 & (w, Gamma) ++ G1) by
+assert (exists Gamma', exists G0, exists G1,
+  Gamma' *=* Gamma /\ G' = G0 & (w, Gamma') ++ G1) by
   ( apply PPermut_split_neq with (G':=G) (w:=w') (Gamma := Delta);
-    [ symmetry; transitivity G0 | ]; auto);
-destruct H3 as [GH]; destruct H3 as [GT]; subst G';
+    [ symmetry; transitivity G0 | ]; auto).
+destruct H3 as (Gamma', (GH, (GT, (H3a, H3b)))); subst;
+assert ((w0, Gamma0) :: (GH & (w, Gamma') ++ GT) & (w', Delta ++ Delta') ~=~
+  (w0, Gamma0) :: (GH & (w, Gamma) ++ GT) & (w', Delta ++ Delta'))
+by PPermut_simpl;
 assert (G ~=~ GH ++ GT & (w', Delta)) by
   ( apply PPermut_last_rev_simpl with (a:=(w, Gamma));
-    transitivity G0; auto;
-    rew_app in *; transitivity (GH ++ (w, Gamma) :: GT & (w', Delta)); auto;
-    transitivity (GH ++ GT ++ (w, Gamma) :: (w', Delta) :: nil); auto);
+    transitivity G0; auto; rewrite H1; PPermut_simpl);
 apply t_letdia_get_LF with
   (Gamma:=Gamma) (G:=GH ++ GT & (w', Delta ++ Delta'))
   (L_w:=L_w \u used_w_vars ((w0, Gamma0) :: (GH & (w, Gamma) ++ GT) &
@@ -567,36 +575,29 @@ apply t_letdia_get_LF with
   (L_t:=L_t \u used_t_vars ((w0, Gamma0) :: (GH & (w, Gamma) ++ GT) &
     (w', Delta ++ Delta')))(A:=A).
 apply ok_Bg_ppermut with
-  (G:=(w0, Gamma0) :: (GH & (w, Gamma) ++ GT) & (w', Delta ++ Delta'));
-rew_app in *; auto;
-transitivity ((w0, Gamma0) :: (w, Gamma) :: GH ++ GT & (w', Delta ++ Delta'));
-auto;
-transitivity (((w,Gamma) :: GH ++ GT & (w', Delta++Delta')) & (w0, Gamma0));
-[ | rew_app]; auto.
+  (G:=(w0, Gamma0) :: (GH & (w, Gamma') ++ GT) & (w', Delta ++ Delta'));
+rew_app in *; auto; try PPermut_simpl.
 apply PPermut_bg with (G:= (GH ++ GT & (w0, Gamma0)) & (w', Delta ++ Delta'));
 [ | rew_app]; auto;
 apply IHHT with (w1:=w) (Gamma1:=Gamma); auto;
-[ rewrite H3 | ]; rew_app; auto;
+[ rewrite H4 | ]; rew_app; auto;
 rew_app; apply ok_Bg_ppermut with
-  (G:=(w0, Gamma0) :: (GH & (w, Gamma) ++ GT) & (w', Delta ++ Delta')); auto;
-rew_app;
-transitivity ((w0, Gamma0) :: (w, Gamma) :: GH ++ GT & (w', Delta ++ Delta'));
-auto;
-transitivity (((w,Gamma) :: GH ++ GT & (w', Delta++Delta')) & (w0, Gamma0));
-[ | rew_app]; auto.
+  (G:=(w0, Gamma0) :: (GH & (w, Gamma') ++ GT) & (w', Delta ++ Delta')); auto;
+rew_app; try PPermut_simpl.
 intros; destruct H with (v':=v')(w':=w'0) (w1:=w0) (Gamma1:=Gamma0); auto;
 apply PPermut_bg with
   (G:=((w'0, (v', A)::nil) :: GH++GT & (w, Gamma)) & (w', Delta ++ Delta'));
 [ | rew_app]; auto;
-apply H6; rew_app; [constructor | ]; auto;
-[ rewrite H3; rew_app; auto | ];
+apply H7; rew_app; [constructor | ]; auto;
+[ rewrite H4; rew_app; auto | ];
 apply ok_Bg_ppermut with
-  (G:= ((w'0, (v', A) :: nil) ::(w0, Gamma0) :: GH & (w, Gamma) ++ GT) &
+  (G:= ((w'0, (v', A) :: nil) ::(w0, Gamma0) :: GH & (w, Gamma') ++ GT) &
     (w', Delta ++ Delta')); rew_app; auto;
 [ transitivity (((w'0, (v', A) :: nil) ::(w0, Gamma0) :: GH ++GT & (w, Gamma))
   & (w', Delta ++ Delta')); rew_app |
- rew_app in *; apply ok_Bg_fresh_wo_te]; auto.
-rew_app; auto.
+ rew_app in *; apply ok_Bg_fresh_wo_te]; auto; try PPermut_simpl.
+rewrite H3; auto.
+rew_app; PPermut_simpl.
 (* letdia_get 2 *)
 apply t_letdia_get_LF with (G:=G) (Gamma:=Gamma) (A:=A)
   (L_w:=L_w \u used_w_vars (((w0, Gamma0 ++ Gamma') :: G & (w, Gamma))))
@@ -642,7 +643,7 @@ Qed.
    can also do it in any "full" version of this context & background
    Proof: ???
 *)
-(* FIXME *)
+(* FIXME Bug: #33 *)
 Lemma types_weakened:
 forall G w Gamma M A
   (Ok: ok_Bg ((w, Gamma)::G))
@@ -700,7 +701,7 @@ subst; apply types_weakened;
 [eapply ok_Bg_permut_first_tail | ]; eauto.
 constructor;
 [ apply ok_Bg_permut_first_tail with (C:=Gamma0) (x:=v0) (A:=A0) |
-  apply Mem_permut with (L2 := (v0, A0) :: Gamma1) in HT]; auto;
+  apply Mem_permut with (l' := (v0, A0) :: Gamma1) in HT]; auto;
 rewrite Mem_cons_eq in HT; destruct HT; auto;
 inversion H2; subst; elim H1; reflexivity.
 
@@ -718,7 +719,7 @@ apply t_lam_LF with (L:=L \u \{v});
 [ apply ok_Bg_permut_first_tail with (C:=Gamma0) (x:=v) (A:=A0) |
   intros]; auto;
 rewrite notin_union in H2; rewrite notin_singleton in H2; destruct H2;
-unfold open_var in *;
+unfold open_t in *;
 rewrite <- subst_t_comm; auto;
 eapply H; auto;
 permut_simpl || rew_app; eauto.
@@ -727,9 +728,9 @@ apply t_lam_LF with (L:=L \u \{v});
 [ apply ok_Bg_ppermut with (G:=((w0, Gamma0)::G0) & (w', Gamma'));
   [ rewrite H2 |
     rewrite H0 in Ok_Bg; rew_app] |
-  intros]; eauto;
+  intros]; eauto with ok_bg_rew;
 rewrite notin_union in H4; rewrite notin_singleton in H4; destruct H4;
-unfold open_var in *;
+unfold open_t in *;
 rewrite <- subst_t_comm; auto;
 eapply H with (G0:=G0) (w':=w'); eauto;
 assert (emptyEquiv G' ~=~ emptyEquiv (G0 ++ nil & (w0, (v', A) :: Gamma0))) as E
@@ -744,13 +745,14 @@ econstructor;
 [ apply ok_Bg_ppermut with (G:=((w0, Gamma0)::G0) & (w', Gamma'));
   [rewrite H1 | rewrite H in Ok_Bg] |
   eapply IHHT1 |
-  eapply IHHT2]; eauto.
+  eapply IHHT2]; eauto;
+apply ok_Bg_permut_no_last_spec in Ok_Bg; rew_app; auto.
 
 (* box *)
 apply t_box_LF with (L:=L \u used_w_vars (emptyEquiv G & (w0, nil)));
 [ apply ok_Bg_permut_no_last with (v:=v) (A:=A0);
   eapply ok_Bg_permut_last |
-  intros; unfold open_ctx]; eauto;
+  intros; unfold open_w]; eauto;
 rewrite <- subst_order_irrelevant_bound;
 [ eapply H; eauto |
   repeat rewrite emptyEquiv_rewrite];
@@ -762,30 +764,28 @@ apply BackgroundSubsetImpl with (G:=emptyEquiv G); auto;
 rew_app; rewrite emptyEquiv_rewrite_last; simpl; auto;
 rewrite H3;
 apply ok_Bg_fresh_wo; auto;
-apply emptyEquiv_ok in Ok_Bg;
+apply emptyEquiv_ok_Bg in Ok_Bg;
 rewrite emptyEquiv_rewrite in Ok_Bg;
 simpl in *; auto.
 
 apply t_box_LF with
   (L:=L \u used_w_vars(emptyEquiv G0 ++ (w', nil) :: (w0, nil) :: nil));
 [ rewrite H2; rewrite H0 in Ok_Bg |
-  intros; unfold open_ctx; rewrite <- subst_order_irrelevant_bound]; eauto;
+  intros; unfold open_w; rewrite <- subst_order_irrelevant_bound];
+eauto with ok_bg_rew;
 eapply H with (G'' := G'' & (w0, Gamma0)) (G0:=G0 & (w0, Gamma0)) (w'0:=w')
   (Gamma':=Gamma') (A0:=A0); auto;
 repeat rewrite emptyEquiv_rewrite;
-simpl; rew_app;
+simpl; rew_app; try PPermut_simpl;
 apply BackgroundSubsetImpl with (G:=emptyEquiv G0 & (w0, nil));
 [ rewrite H1 in H3; rewrite emptyEquiv_rewrite in H3 |
   exists ((w'0, (@nil (var * ty)))::nil); rew_app |
-  apply emptyEquiv_ok in Ok_Bg; rewrite H0 in Ok_Bg]; auto;
+  apply emptyEquiv_ok_Bg in Ok_Bg; rewrite H0 in Ok_Bg]; auto;
 repeat rewrite emptyEquiv_rewrite in Ok_Bg;
 simpl in *; rew_app in *;
 apply ok_Bg_ppermut with
   (G:=(w'0, nil) :: emptyEquiv G0 ++ (w', nil) :: (w0, nil) :: nil);
-[ transitivity ((w', nil) :: (w'0, nil):: emptyEquiv G0 & (w0, nil)); auto;
-  transitivity ((w'0, nil) :: (w', nil) :: emptyEquiv G0 & (w0, nil)) |
-    apply ok_Bg_fresh_wo];
-auto.
+[eauto with ppermut_rew | apply ok_Bg_fresh_wo ]; auto.
 
 (* unbox *)
 econstructor; [ | eapply IHHT];
@@ -793,7 +793,7 @@ try apply ok_Bg_permut_first_tail with (C:=Gamma0) (x:=v) (A:=A0); eauto.
 
 econstructor;
 [ rewrite H1; rewrite H in Ok_Bg |
-  eapply IHHT]; eauto.
+  eapply IHHT]; eauto with ok_bg_rew.
 
 (* unbox_fetch *)
 apply t_unbox_fetch_LF with (G:=G) (Gamma:=Gamma); auto;
@@ -805,39 +805,46 @@ destruct (eq_var_dec w w'0).
 (* = *)
 subst;
 assert (G ~=~ G0 /\ Gamma *=* (v, A0) :: Gamma'0) as HP by
-  (apply ok_Bg_impl_ppermut with (w:=w'0); eauto);
+  (apply ok_Bg_impl_ppermut with (w:=w'0);
+   [eauto with ok_bg_rew | transitivity G'; auto]);
 destruct HP;
 apply t_unbox_fetch_LF with (G:=G) (Gamma:=Gamma'0);
-eauto;
+eauto with ok_bg_rew;
 specialize IHHT with (Gamma1:=Gamma) (w:=w'0);
 destruct IHHT with (M0:=M0) (A0:=A0) (v:=v); auto;
-apply H6; eauto;
-rewrite H1 in H3; rewrite H4; auto.
+[ apply H6; eauto; rewrite H1 in H3; rewrite H4 |
+  rewrite H4; symmetry]; auto.
 (* <> *)
-assert (exists GH, exists GT, G = GH & (w'0, (v, A0)::Gamma'0) ++ GT) as HP by
-  (apply PPermut_split_neq with (w:=w) (Gamma:=Gamma) (G':=G0); eauto);
-destruct HP as (GH, HP); destruct HP as (GT, HP);
+assert (exists Gamma', exists GH, exists GT,
+  Gamma' *=* (v, A0)::Gamma'0 /\ G = GH & (w'0, Gamma') ++ GT) as HP by
+  (apply PPermut_split_neq with (w:=w) (Gamma:=Gamma) (G':=G0);
+    eauto; transitivity G'; auto).
+destruct HP as (Gamma', (GH, (GT, (HPa, HPb)))).
+assert (GH & (w'0, Gamma') ++ GT ~=~ GH & (w'0, (v, A0)::Gamma'0) ++ GT)
+  by PPermut_simpl;
 apply t_unbox_fetch_LF with (G:=GH ++ GT & (w'0, Gamma'0)) (Gamma:=Gamma).
 subst;
 apply ok_Bg_ppermut with
   (G:= (((w, Gamma) :: (GH & (w0, Gamma0) ++ GT)) & (w'0, Gamma'0)));
 [rew_app | ]; auto;
-apply ok_Bg_permut_no_last_spec with (v:=v)(A:=A0);
+apply ok_Bg_permut_no_last_spec with (v:=v)(A:=A0).
 apply ok_Bg_ppermut with
-  (G:=(w, Gamma):: (GH & (w'0, (v, A0) :: Gamma'0) ++ GT) & (w0, Gamma0));
-rew_app in *; auto.
+  (G:=(w, Gamma):: (GH & (w'0, Gamma') ++ GT) & (w0, Gamma0));
+rew_app in *; auto; PPermut_simpl.
 eapply IHHT with (w1:=w) (Gamma1:=Gamma) (w':=w'0) (Gamma':=Gamma'0)
                  (G0:=GH ++ GT & (w0, Gamma0)); rew_app; auto; subst;
 rew_app; auto;
 rewrite H1 in H3;
 assert (GH ++ (w, Gamma) :: GT ~=~ G0) by
   (apply PPermut_last_rev_simpl with (a:=(w'0, (v, A0) :: Gamma'0));
-  rew_app in *; rewrite <- H0; rewrite <- H; auto);
+  rew_app in *; rewrite <- H0; rewrite <- H; auto; PPermut_simpl).
+PPermut_simpl; eauto.
 assert (GH ++ (w, Gamma) :: GT & (w0, Gamma0) ~=~ G0 & (w0,Gamma0)) by
-  (rewrite <- H4; rew_app; auto);
-rewrite H5; auto.
-subst; rew_app in *;
-transitivity (G0 & (w'0, Gamma'0)); [ | symmetry]; eauto.
+  (rewrite <- H5; rew_app; auto; PPermut_simpl);
+rewrite H6; auto.
+subst; rewrite H2; PPermut_simpl.
+apply PPermut_last_rev with (w:=w'0) (Gamma:=Gamma') (Gamma':=(v,A0)::Gamma'0);
+[ | symmetry]; auto; transitivity G'; auto; rewrite <- H; PPermut_simpl.
 
 (* here *)
 econstructor; [ | eapply IHHT];
@@ -845,7 +852,7 @@ try apply ok_Bg_permut_first_tail with (C:=Gamma0) (x:=v) (A:=A0); eauto.
 
 econstructor;
 [ rewrite H1; rewrite H in Ok_Bg |
-  eapply IHHT]; eauto.
+  eapply IHHT]; eauto with ok_bg_rew.
 
 (* get_here *)
 apply t_get_here_LF with (G:=G) (Gamma:=Gamma); auto;
@@ -853,43 +860,50 @@ apply t_get_here_LF with (G:=G) (Gamma:=Gamma); auto;
   apply ok_Bg_ppermut with (G:= (w, Gamma) :: G & (w0, Gamma0)) |
   eapply IHHT; eauto; rewrite <- H in H1; rew_app]; auto.
 
-destruct (eq_var_dec w w').
+destruct (eq_var_dec w w'0).
 (* = *)
 subst;
-assert (G ~=~ G0 /\ Gamma *=* (v, A0) :: Gamma') as HP by
-  (apply ok_Bg_impl_ppermut with (w:=w'); eauto);
+assert (G ~=~ G0 /\ Gamma *=* (v, A0) :: Gamma'0) as HP by
+  (apply ok_Bg_impl_ppermut with (w:=w'0);
+   [eauto with ok_bg_rew | transitivity G'; auto]);
 destruct HP;
-apply t_get_here_LF with (G:=G) (Gamma:=Gamma');
-eauto;
-specialize IHHT with (Gamma1:=Gamma) (w:=w');
+apply t_get_here_LF with (G:=G) (Gamma:=Gamma'0);
+eauto with ok_bg_rew;
+specialize IHHT with (Gamma1:=Gamma) (w:=w'0);
 destruct IHHT with (M0:=M0) (A0:=A0) (v:=v); auto;
-apply H7; eauto;
-rewrite H1 in H3; rewrite H5; auto.
+[ apply H6; eauto; rewrite H1 in H3; rewrite H4 |
+  rewrite H4; symmetry]; auto.
 (* <> *)
-assert (exists GH, exists GT, G = GH & (w', (v, A0)::Gamma') ++ GT) as HP by
-  (apply PPermut_split_neq with (w:=w) (Gamma:=Gamma) (G':=G0); eauto);
-destruct HP as (GH, HP); destruct HP as (GT, HP);
-apply t_get_here_LF with (G:=GH ++ GT & (w', Gamma')) (Gamma:=Gamma).
+assert (exists Gamma', exists GH, exists GT,
+  Gamma' *=* (v, A0)::Gamma'0 /\ G = GH & (w'0, Gamma') ++ GT) as HP by
+  (apply PPermut_split_neq with (w:=w) (Gamma:=Gamma) (G':=G0);
+    eauto; transitivity G'; auto).
+destruct HP as (Gamma', (GH, (GT, (HPa, HPb)))).
+assert (GH & (w'0, Gamma') ++ GT ~=~ GH & (w'0, (v, A0)::Gamma'0) ++ GT)
+  by PPermut_simpl;
+apply t_get_here_LF with (G:=GH ++ GT & (w'0, Gamma'0)) (Gamma:=Gamma).
 subst;
 apply ok_Bg_ppermut with
-  (G:= (((w, Gamma) :: (GH & (w0, Gamma0) ++ GT)) & (w', Gamma')));
+  (G:= (((w, Gamma) :: (GH & (w0, Gamma0) ++ GT)) & (w'0, Gamma'0)));
 [rew_app | ]; auto;
-apply ok_Bg_permut_no_last_spec with (v:=v)(A:=A0);
+apply ok_Bg_permut_no_last_spec with (v:=v)(A:=A0).
 apply ok_Bg_ppermut with
-  (G:=(w, Gamma):: (GH & (w', (v, A0) :: Gamma') ++ GT) & (w0, Gamma0));
-rew_app in *; auto.
-eapply IHHT with (w1:=w) (Gamma1:=Gamma) (w':=w') (Gamma':=Gamma')
+  (G:=(w, Gamma):: (GH & (w'0, Gamma') ++ GT) & (w0, Gamma0));
+rew_app in *; auto; PPermut_simpl.
+eapply IHHT with (w1:=w) (Gamma1:=Gamma) (w':=w'0) (Gamma':=Gamma'0)
                  (G0:=GH ++ GT & (w0, Gamma0)); rew_app; auto; subst;
 rew_app; auto;
 rewrite H1 in H3;
 assert (GH ++ (w, Gamma) :: GT ~=~ G0) by
-  (apply PPermut_last_rev_simpl with (a:=(w', (v, A0) :: Gamma'));
-  rew_app in *; rewrite <- H0; rewrite <- H; auto);
+  (apply PPermut_last_rev_simpl with (a:=(w'0, (v, A0) :: Gamma'0));
+  rew_app in *; rewrite <- H0; rewrite <- H; auto; PPermut_simpl).
+PPermut_simpl; eauto.
 assert (GH ++ (w, Gamma) :: GT & (w0, Gamma0) ~=~ G0 & (w0,Gamma0)) by
-  (rewrite <- H5; rew_app; auto);
+  (rewrite <- H5; rew_app; auto; PPermut_simpl);
 rewrite H6; auto.
-subst; rew_app in *;
-transitivity (G0 & (w', Gamma')); [ | symmetry]; eauto.
+subst; rewrite H2; PPermut_simpl.
+apply PPermut_last_rev with (w:=w'0) (Gamma:=Gamma') (Gamma':=(v,A0)::Gamma'0);
+[ | symmetry]; auto; transitivity G'; auto; rewrite <- H; PPermut_simpl.
 
 (* letdia *)
 apply t_letdia_LF with
@@ -898,35 +912,36 @@ apply t_letdia_LF with
 [ apply ok_Bg_permut_first_tail with (C:=Gamma0) (x:=v) (A:=A0) |
   eapply IHHT |
   intros]; eauto;
-unfold open_var in *; unfold open_ctx in *;
+unfold open_t in *; unfold open_w in *;
 rewrite notin_union in H2; rewrite notin_singleton in H2; destruct H2;
 rewrite <- subst_order_irrelevant_bound;
 [ rewrite <- subst_t_comm | assumption ];
 [ eapply H | |] ; eauto;
 apply BackgroundSubsetImpl with (G:=emptyEquiv G); auto;
-[ eauto | ];
+[ exists ((w', (@nil (var*ty)))::nil);
+  PPermut_simpl ; rew_app; PPermut_simpl | ].
 assert ((w0, nil) :: (w', nil) :: emptyEquiv G ~=~
-  (w',nil) :: (w0, nil) :: emptyEquiv G) by auto;
+  (w',nil) :: (w0, nil) :: emptyEquiv G) by PPermut_simpl;
 rewrite H5; apply ok_Bg_fresh_wo;
-[ apply emptyEquiv_ok in Ok_Bg;  simpl in * | ]; auto.
+[ apply emptyEquiv_ok_Bg in Ok_Bg;  simpl in * | ]; auto.
 
 eapply t_letdia_LF with
   (L_t := L_t \u \{v})
   (L_w := L_w \u  used_w_vars ((w', nil) :: emptyEquiv (G0 & (w0, Gamma0))));
-[ rewrite H2; rewrite H0 in Ok_Bg | eapply IHHT | intros]; eauto;
-unfold open_var in *; unfold open_ctx in *;
+[ rewrite H2; rewrite H0 in Ok_Bg | eapply IHHT | intros]; eauto with ok_bg_rew;
+unfold open_t in *; unfold open_w in *.
 rewrite notin_union in H4; rewrite notin_singleton in H4; destruct H4;
 rewrite <- subst_order_irrelevant_bound;
 [ rewrite <- subst_t_comm | assumption ];
 [ eapply H with (G0:=(w'0, (v',A)::nil)::G0) (w'0:=w')
   (Gamma':=Gamma') (A0:=A0) | | ]; eauto;
-rew_app; rewrite H1 in H3; rew_app in *; simpl;
+rew_app; rewrite H1 in H3; rew_app in *; simpl; try PPermut_simpl;
 apply BackgroundSubsetImpl with (G:= emptyEquiv (G0 & (w0, Gamma0))); auto;
-[eauto | ];
+[exists ((w'0, (@nil (var*ty))):: nil); PPermut_simpl | ];
 assert ((w'0, nil) :: (w', nil)::emptyEquiv(G0 & (w0, Gamma0)) ~=~
   (w', nil) :: (w'0, nil) :: emptyEquiv (G0 & (w0, Gamma0))) by auto;
 rewrite <- H7; apply ok_Bg_fresh_wo;
-[rewrite H0 in Ok_Bg; apply emptyEquiv_ok in Ok_Bg | ]; auto;
+[rewrite H0 in Ok_Bg; apply emptyEquiv_ok_Bg in Ok_Bg | ]; auto;
   assert (emptyEquiv((w', (v, A0) :: Gamma') :: G0 & (w0, Gamma0)) ~=~
     (w', nil) :: emptyEquiv (G0 & (w0, Gamma0))) by (simpl; auto);
 rewrite <- H8;
@@ -935,120 +950,126 @@ assert ((w0, Gamma0) :: G0 & (w', (v, A0) :: Gamma') ~=~
 rewrite <- H9; auto.
 
 (* letdia_get *)
-assert (w <> w0) by eauto;
+assert (w <> w0) by eauto with ok_bg_rew;
 eapply t_letdia_get_LF with (G:=G) (Gamma:=Gamma) (L_t := L_t \u \{v})
   (L_w:=L_w \u used_w_vars ((w0, nil) :: emptyEquiv (G & (w, Gamma)))); auto.
 apply ok_Bg_permut_no_last_spec with (v:=v) (A:=A0);
 apply ok_Bg_ppermut with (G:= (w, Gamma) :: G & (w0, Gamma0)); auto.
 eapply IHHT; eauto.
 rew_app; rewrite <- H0 in H2; auto.
-intros; unfold open_var in *; unfold open_ctx in *;
+intros; unfold open_t in *; unfold open_w in *;
 rewrite notin_union in H5; rewrite notin_singleton in H5; destruct H5;
 rewrite <- subst_order_irrelevant_bound;
 [rewrite <- subst_t_comm | ]; auto;
 eapply H; eauto;
 rewrite <- H0 in H2;
 apply BackgroundSubsetImpl with (G:=emptyEquiv (G & (w, Gamma))); auto;
-[ eauto | ];
+[ exists ((w', (@ nil (var * ty)))::nil); PPermut_simpl | ];
 assert ((w0, nil) :: (w', nil) :: emptyEquiv (G & (w, Gamma)) ~=~
-  (w', nil) :: (w0, nil) ::emptyEquiv (G & (w, Gamma))); auto;
+  (w', nil) :: (w0, nil) ::emptyEquiv (G & (w, Gamma))) by PPermut_simpl;
 rewrite H8;
-apply ok_Bg_fresh_wo; [apply emptyEquiv_ok in Ok_Bg | auto];
+apply ok_Bg_fresh_wo; [apply emptyEquiv_ok_Bg in Ok_Bg | auto];
 assert ((w, Gamma) :: G & (w0, Gamma0) ~=~ (w0, Gamma0):: G & (w, Gamma)) by
   auto;
 rewrite H9 in Ok_Bg; simpl in Ok_Bg; auto.
 
-assert (w <> w0) by eauto;
+assert (w <> w0) by eauto with ok_bg_rew;
 destruct (eq_var_dec w w'); subst.
 (* = *)
 assert (G ~=~ G1 /\ Gamma *=* (v, A0) :: Gamma') by
   (apply ok_Bg_impl_ppermut with (w:=w');
     [ | rewrite H0; rewrite <- H1]; eauto);
-destruct H7;
+destruct H7; rewrite H3; rewrite <- H7;
 eapply t_letdia_get_LF with (G:=G) (Gamma:=Gamma') (L_t:=L_t \u \{v})
-  (L_w:=L_w \u used_w_vars ((w', nil) :: emptyEquiv (G1 & (w0, Gamma0)))); auto;
-[eauto | eapply IHHT; eauto; rewrite H2 in H4; rewrite H7; auto | | ].
-intros; unfold open_var in *; unfold open_ctx in *;
+  (L_w:=L_w \u used_w_vars ((w', nil) :: emptyEquiv (G1 & (w0, Gamma0))));
+[ eauto with ok_bg_rew |
+  eapply IHHT; eauto; rewrite H2 in H4; rewrite H7 | | ]; auto.
+intros; unfold open_t in *; unfold open_w in *;
 rewrite notin_union in H9; rewrite notin_singleton in H9; destruct H9;
 rewrite <- subst_order_irrelevant_bound;
-[ rewrite <- subst_t_comm | ]; auto;
-eapply H with (v:=v); eauto; rew_app;
-rewrite H2 in H4; rewrite H7;
+[ rewrite <- subst_t_comm | ]; auto.
+edestruct H with (v:=v) (w'0 := w'0) (Gamma1:=Gamma0) (A0:=A0) as (Ha, Hb);
+eauto;
+eapply Hb with (G0 := (w'0, (v',A)::nil) ::G) (w'1 := w') (Gamma':=Gamma');
+[ | eauto |  | ]; try PPermut_simpl.
+rewrite H2 in H4; rewrite H7.
 apply BackgroundSubsetImpl with (G:=emptyEquiv (G1 & (w0, Gamma0))); auto.
-exists (((w'0, (@nil (prod var ty))) :: nil)); rew_app; simpl; auto.
+exists (((w'0, (@nil (prod var ty))) :: nil)); rew_app; simpl; auto;
+PPermut_simpl.
 assert ((w', nil) :: (w'0, nil) :: emptyEquiv (G1 & (w0, Gamma0)) ~=~
   (w'0, nil) :: (w',nil) :: emptyEquiv (G1 & (w0, Gamma0))) by auto;
 rewrite H12; apply ok_Bg_fresh_wo; auto;
 assert ((w', nil) :: emptyEquiv (G1 & (w0, Gamma0)) ~=~
   emptyEquiv ((w', Gamma) :: G & (w0, Gamma0))) by
   (simpl in *; rewrite H7; auto);
-rewrite H13; apply emptyEquiv_ok in Ok_Bg; auto.
-symmetry; rewrite H7; auto.
+rewrite H13; apply emptyEquiv_ok_Bg in Ok_Bg; auto.
 (* <> *)
 assert (G & (w, Gamma) ~=~ G1 & (w', (v, A0) :: Gamma')) by
   (transitivity G0; auto);
 symmetry in H7;
-assert (exists GH, exists GT, G1 = GH & (w, Gamma) ++ GT) by
+assert (exists Gamma0, exists GH, exists GT,
+  Gamma0 *=* Gamma /\ G1 = GH & (w, Gamma0) ++ GT) by
   (apply PPermut_split_neq with (w:=w') (Gamma:=(v,A0) :: Gamma') (G':=G);
     auto);
-destruct H8 as (GH, H8); destruct H8 as (GT, H8);
+destruct H8 as (Gamma'', (GH, H8)); destruct H8 as (GT, H8);
+destruct H8.
 eapply t_letdia_get_LF with (G:=GH++GT & (w', Gamma')) (Gamma:=Gamma)
   (L_t:=L_t \u \{v}) (L_w:=L_w \u used_w_vars
      ((w', nil) :: emptyEquiv (GH ++ GT ++ (w, Gamma) :: (w0, Gamma0) :: nil))).
 assert (G & (w, Gamma) & (w0, Gamma0) ~=~ (w, Gamma) :: G & (w0, Gamma0)) by
-  auto;
-rewrite <- H9 in Ok_Bg; rewrite <- H7 in Ok_Bg; rewrite H8 in Ok_Bg;
+  auto.
+rewrite <- H10 in Ok_Bg; rewrite <- H7 in Ok_Bg;
 subst; apply ok_Bg_ppermut with
   (G:=((w, Gamma) :: (GH & (w', Gamma') ++ GT) & (w0, Gamma0))); [ | rew_app];
-auto;
+auto.
 apply ok_Bg_ppermut with
   (G:= (((w, Gamma) :: (GH & (w0, Gamma0) ++ GT)) & (w', Gamma')));
-[rew_app; auto | apply ok_Bg_permut_no_last_spec with (v:=v)(A:=A0)];
+[rew_app; PPermut_simpl | apply ok_Bg_permut_no_last_spec with (v:=v)(A:=A0)];
 apply ok_Bg_ppermut with
-  ((GH & (w, Gamma) ++ GT) & (w', (v, A0) :: Gamma') & (w0, Gamma0));
-[ rew_app | ]; auto.
+  ((GH & (w, Gamma'') ++ GT) & (w', (v, A0) :: Gamma') & (w0, Gamma0));
+[ rew_app | ]; auto; try PPermut_simpl.
 eapply IHHT with (w1:=w) (Gamma1:=Gamma) (A0:=A0) (w':=w')
   (G0:=GH++GT & (w0,Gamma0)) (Gamma':=Gamma'); auto;
-[ symmetry; subst; rew_app in * | rew_app | ]; eauto;
-rewrite H2 in H4; rewrite H8 in H4;
-assert ((GH & (w, Gamma) ++ GT) & (w0, Gamma0) ~=~
-  (GH ++ GT & (w0, Gamma0)) ++ nil & (w, Gamma)) by (rew_app; auto);
-rewrite <- H9; auto.
-intros; unfold open_var in *; unfold open_ctx in *;
-rewrite notin_union in H9; rewrite notin_singleton in H9; destruct H9;
+[ symmetry; subst; rew_app in * | rew_app | ]; eauto.
+PPermut_simpl; apply PPermut_last_rev_simpl with (a:=(w, Gamma));
+rewrite <- H7; PPermut_simpl.
+rewrite H2 in H4; rewrite H9 in H4;
+assert ((GH & (w, Gamma'') ++ GT) & (w0, Gamma0) ~=~
+  (GH ++ GT & (w0, Gamma0)) ++ nil & (w, Gamma)) by (rew_app; PPermut_simpl);
+rewrite <- H10; auto.
+intros; unfold open_t in *; unfold open_w in *;
+rewrite notin_union in H10; rewrite notin_singleton in H10; destruct H10;
 rewrite <- subst_order_irrelevant_bound;
 [rewrite <- subst_t_comm | ]; auto;
 eapply H with (v':=v') (w':=w'0) (Gamma1:=Gamma0) (w1:=w0) (A0:=A0)
               (v:=v) (G0:=(w'0, (v', A) :: nil) :: (GH ++ GT) & (w, Gamma))
-              (w'0:=w') (Gamma':=Gamma'); auto.
-rew_app; constructor; auto.
-symmetry; transitivity (G1 & (w', (v, A0) :: Gamma')); auto;
-subst; rew_app; auto.
-rew_app; constructor; auto.
-rew_app; rewrite H2 in H4; rewrite H8 in H4; simpl;
+              (w'0:=w') (Gamma':=Gamma'); auto; try PPermut_simpl.
+apply PPermut_last_rev_simpl with (a:=(w, Gamma)); rewrite <- H7;
+subst; PPermut_simpl.
+rew_app; rewrite H2 in H4; rewrite H9 in H4; simpl;
 apply BackgroundSubsetImpl with
   (G:=emptyEquiv (GH ++ GT ++ (w, Gamma) :: (w0, Gamma0) :: nil)); auto.
 assert (GH ++ GT ++ (w, Gamma) :: (w0, Gamma0) :: nil ~=~
-  (GH & (w, Gamma) ++ GT) & (w0, Gamma0)) by (rew_app; auto);
-rewrite H12; auto.
-eauto.
+  (GH & (w, Gamma'') ++ GT) & (w0, Gamma0)) by (rew_app; PPermut_simpl);
+rewrite H13; auto.
+exists ((w'0, (@nil (var*ty))) :: nil); PPermut_simpl.
 assert ((w, Gamma) :: G & (w0, Gamma0) ~=~ G0 & (w0, Gamma0)) by
   (rewrite <- H0; auto);
-rewrite H12 in Ok_Bg; rewrite H1 in Ok_Bg; subst;
+rewrite H13 in Ok_Bg; rewrite H1 in Ok_Bg; subst;
 assert ((w', nil)
       :: (w'0, nil)
          :: emptyEquiv (GH ++ GT ++ (w, Gamma) :: (w0, Gamma0) :: nil) ~=~
       (w'0, nil)
       :: (w', nil)
          :: emptyEquiv (GH ++ GT ++ (w, Gamma) :: (w0, Gamma0) :: nil)) by auto;
-rewrite H8; apply ok_Bg_fresh_wo;
-assert ( ((GH & (w, Gamma) ++ GT) & (w', (v, A0) :: Gamma')) & (w0, Gamma0) ~=~
+rewrite H9; apply ok_Bg_fresh_wo;
+assert (((GH & (w, Gamma'') ++ GT) & (w', (v, A0) :: Gamma')) & (w0, Gamma0) ~=~
   ((w', (v, A0) :: Gamma') :: GH ++ GT ++ (w, Gamma) :: nil) &  (w0, Gamma0)) by
-  (eapply PPermut_last; auto);
-rew_app in *; [rewrite H13 in Ok_Bg | auto];
-apply emptyEquiv_ok in Ok_Bg; simpl in *; auto.
-symmetry; transitivity (G1 & (w', Gamma')); subst; rew_app in *; auto.
-Qed.
+  (eapply PPermut_last_rev; auto; try PPermut_simpl);
+rew_app in *; [rewrite H14 in Ok_Bg | auto];
+apply emptyEquiv_ok_Bg in Ok_Bg; simpl in *; auto.
+symmetry; transitivity (G1 & (w', Gamma')); subst; rew_app in *; PPermut_simpl.
+Admitted. (* No more subgoals but non-instantiated existential variables: 4 *)
 
 Lemma subst_t_preserv_types_inner:
 forall G w Gamma A B M N v
@@ -1106,22 +1127,24 @@ simpl in *.
 (* hyp *)
 constructor;
 [ rewrite H in Ok_Bg  |
-  rewrite Mem_app_or_eq; left ]; eauto.
+  rewrite Mem_app_or_eq; left ]; auto;
+eapply ok_Bg_split2; eauto.
 constructor;
 [ rewrite H in Ok_Bg |
-  rewrite Mem_app_or_eq; right ]; eauto.
+  rewrite Mem_app_or_eq; right ]; auto;
+eapply ok_Bg_split2; eauto.
 constructor;
-[ rewrite H in Ok_Bg; rewrite H0 | ]; eauto.
-
+[ rewrite H in Ok_Bg; rewrite H0 | ]; auto;
+eapply ok_Bg_split3; eauto.
 (* lam *)
 apply t_lam_LF with (L := L);
-[ rewrite H0 in Ok_Bg; eauto |
-  intros; unfold open_var in *];
+[ rewrite H0 in Ok_Bg; eapply ok_Bg_split2; eauto |
+  intros; unfold open_t in *];
 rewrite subst_order_irrelevant_free; simpl; auto;
 apply H with (v':=v') (G':=G') (Gamma := (v',A)::Gamma0); auto.
 apply t_lam_LF with (L := L);
-[ rewrite H0 in Ok_Bg; eauto |
-  intros]; unfold open_var in *;
+[ rewrite H0 in Ok_Bg; eapply ok_Bg_split2; eauto |
+  intros]; unfold open_t in *;
 rewrite subst_order_irrelevant_free;
 edestruct H; eauto; destruct H3;
 [ apply ContextPermutImpl with (Gamma := (Gamma' ++ (v', A) :: Gamma0));
@@ -1129,8 +1152,8 @@ edestruct H; eauto; destruct H3;
 apply t_lam_LF with (L := L);
 [ rewrite H0 in Ok_Bg |
   intros];
-rewrite H1; eauto;
-unfold open_var in *;
+rewrite H1; try eapply ok_Bg_split3; eauto;
+unfold open_t in *;
 rewrite subst_order_irrelevant_free;
 edestruct H; eauto; destruct H4;
 eauto;
@@ -1141,55 +1164,59 @@ apply t_appl_LF with (A:=A);
 [ rewrite H in Ok_Bg |
   apply IHHT1 with (Gamma:=Gamma0) |
   apply IHHT2 with (Gamma:=Gamma0) ];
-eauto.
+eauto; eapply ok_Bg_split2; eauto.
 apply t_appl_LF with (A:=A);
 [ rewrite H in Ok_Bg |
   apply IHHT1 with (Gamma:=Gamma0) |
   apply IHHT2 with (Gamma:=Gamma0) ];
-eauto.
+eauto; eapply ok_Bg_split2; eauto.
 apply t_appl_LF with (A:=A);
 [ rewrite H in Ok_Bg; rewrite H0 |
   eapply IHHT1 |
-  eapply IHHT2 ]; eauto.
+  eapply IHHT2 ]; eauto;
+eapply ok_Bg_split3; eauto.
 
 (* box *)
 apply t_box_LF with (L:=\{w'} \u L);
-[ rewrite H0 in Ok_Bg; eauto |
+[ rewrite H0 in Ok_Bg; eapply ok_Bg_split4; eauto |
   intros];
-unfold open_ctx in *; rewrite notin_union in H1; destruct H1;
+unfold open_w in *; rewrite notin_union in H1; destruct H1;
 rewrite notin_singleton in *; rewrite <- subst_w_comm; auto;
-eapply H; eauto.
+eapply H; eauto; PPermut_simpl.
 apply t_box_LF with (L:=\{w0} \u L);
 [ rewrite H0 in Ok_Bg; apply ok_Bg_split4 with (w:=w0);
   apply ok_Bg_ppermut with (G:=G' & (w', Gamma') & (w0, Gamma0)); auto |
-  intros];
-unfold open_ctx in *; rewrite notin_union in H1; destruct H1;
+  intros]; try PPermut_simpl;
+unfold open_w in *; rewrite notin_union in H1; destruct H1;
 rewrite notin_singleton in *; rewrite <- subst_w_comm; auto;
 eapply H; eauto.
 apply t_box_LF with (L:=\{w''} \u L);
-[ rewrite H0 in Ok_Bg; rewrite H1; eauto |
+[ rewrite H0 in Ok_Bg; rewrite H1; eapply ok_Bg_split6; eauto |
   intros];
-unfold open_ctx in *;
+unfold open_w in *;
 rewrite notin_union in H2; destruct H2;
 rewrite notin_singleton in *;
 rewrite <- subst_w_comm; auto;
 eapply H with (G0:=G0 & (w0, Gamma0)) (Gamma':=Gamma') (Gamma'':=Gamma''); auto;
-rewrite H0; auto.
+try PPermut_simpl; rewrite H0; PPermut_simpl.
 
 (* unbox *)
 case_if.
 inversion H0; subst; rewrite H in Ok_Bg;
 apply ok_Bg_first_last_neq in Ok_Bg; elim Ok_Bg; auto.
-constructor; [rewrite H in Ok_Bg | apply IHHT with (Gamma:=Gamma0)]; eauto.
+constructor; [rewrite H in Ok_Bg | apply IHHT with (Gamma:=Gamma0)]; eauto;
+eapply ok_Bg_split2; eauto.
 
 case_if; constructor;
 [ rewrite H in Ok_Bg |
-  apply IHHT with (Gamma:=Gamma0) ]; eauto.
+  apply IHHT with (Gamma:=Gamma0) ]; eauto;
+eapply ok_Bg_split2; eauto.
 
 case_if.
 inversion H1; subst; rewrite H in Ok_Bg;
 apply ok_Bg_first_last_neq in Ok_Bg; elim Ok_Bg; auto.
-constructor; [rewrite H0; rewrite H in Ok_Bg | eapply IHHT]; eauto.
+constructor; [rewrite H0; rewrite H in Ok_Bg | eapply IHHT]; eauto;
+eapply ok_Bg_split3; eauto.
 
 (* unbox_fetch *)
 case_if.
@@ -1205,21 +1232,29 @@ apply ContextPermutImpl with (Gamma:=Gamma0 ++ Gamma);
   apply IHHT] ; auto.
 assert (G'0 & (w'0, Gamma'0) ~=~ G & (w, Gamma)) by
   (symmetry; transitivity G'; auto);
-assert (exists GH, exists GT, G'0 = GH & (w, Gamma) ++ GT) as Split by
+assert (exists Gamma'', exists GH, exists GT,
+  Gamma'' *=* Gamma /\ G'0 = GH & (w, Gamma'') ++ GT) as Split by
   (eapply PPermut_split_neq; eauto; right; intro; subst; elim H1; reflexivity);
-destruct Split as (GH, Split); destruct Split as (GT); subst;
+destruct Split as (Gamma'', (GH, Split)); destruct Split as (GT, H3);
+destruct H3 as (H3a, H3b).
 apply t_unbox_fetch_LF with (G:=GH++GT) (Gamma:=Gamma).
 assert ((w, Gamma) :: G & (w0, Gamma0) ~=~ G & (w, Gamma) & (w0, Gamma0)) by
-  auto;
+  auto.
 rewrite H3 in Ok_Bg; rewrite <- H2 in Ok_Bg; rew_app in *;
-assert (GH & (w, Gamma) ++ GT ~=~ (w, Gamma) :: GH ++ GT) by (symmetry; eauto);
+assert (GH & (w, Gamma) ++ GT ~=~ (w, Gamma) :: GH ++ GT) by (PPermut_simpl);
 apply ok_Bg_ppermut with
   (G:= (GH & (w, Gamma) ++ GT) & (w0, Gamma0 ++ Gamma'0));
 [ rewrite H4 |
   apply ok_Bg_split4 with (w:=w'0)]; rew_app; auto.
-eapply IHHT with (w1:=w) (Gamma1:=Gamma); auto.
-apply PPermut_last_rev_simpl with (a:=(w, Gamma)); rew_app in *; auto.
-rew_app; auto.
+subst; rew_app in *;
+apply ok_Bg_ppermut with
+  (G:=(GH ++ (w, Gamma'') :: GT ++ (w'0, Gamma'0) :: (w0, Gamma0) :: nil));
+try PPermut_simpl; auto.
+eapply IHHT with (w1:=w) (Gamma1:=Gamma); auto; subst; symmetry; PPermut_simpl;
+apply PPermut_last_rev_simpl with (a:=(w, Gamma)); rew_app in *; auto;
+rew_app; auto; rewrite <- H2; PPermut_simpl.
+apply PPermut_last_rev_simpl with (a:=(w, Gamma)); rew_app in *; auto; subst;
+PPermut_simpl.
 
 case_if;
 [ inversion H1; subst; apply ok_Bg_first_last_neq in Ok_Bg; elim Ok_Bg; auto |
@@ -1227,32 +1262,35 @@ case_if;
 subst; assert (G ~=~ G'0 /\ Gamma *=* Gamma'0) by
   (apply ok_Bg_impl_ppermut with (w:=w'0); [ | rewrite <- H0]; eauto);
 destruct H2; constructor.
-rewrite <- H2; apply ok_Bg_permut with (Ctx := (Gamma ++ Gamma0)); eauto.
+rewrite <- H2; apply ok_Bg_permut with (Ctx := (Gamma ++ Gamma0)); eauto;
+eapply ok_Bg_split2; eauto.
 apply ContextPermutImpl with (Gamma:=Gamma ++ Gamma0);
 [ permut_simpl |
   eapply IHHT with (w:=w'0) (Gamma1:=Gamma) (Gamma':=Gamma0)] ; auto.
 assert (G'0 & (w'0, Gamma'0) ~=~ G & (w, Gamma)) by
   (symmetry; transitivity G'; auto);
-assert (exists GH, exists GT, G'0 = GH & (w, Gamma) ++ GT) as Split by
+assert (exists Gamma'', exists GH, exists GT,
+  Gamma'' *=* Gamma /\ G'0 = GH & (w, Gamma'') ++ GT) as Split by
   (eapply PPermut_split_neq; eauto; right; intro; subst; elim H1; reflexivity);
-destruct Split as (GH, Split); destruct Split as (GT); subst;
+destruct Split as (Gamma'', (GH, Split));
+destruct Split as (GT, (Ha, Hb)); subst;
 apply t_unbox_fetch_LF with (G:=GH++GT) (Gamma:=Gamma).
-assert (GH & (w, Gamma) ++ GT ~=~ (w, Gamma) :: GH ++ GT) by (symmetry; eauto);
+assert (GH & (w, Gamma) ++ GT ~=~ (w, Gamma) :: GH ++ GT)
+  by PPermut_simpl;
 apply ok_Bg_ppermut with
-  (G:= (GH & (w, Gamma) ++ GT) & (w'0, Gamma0 ++ Gamma'0));
-[ rewrite H3 | apply ok_Bg_split4 with (w:=w0)]; rew_app; auto;
+  (G:= (GH & (w, Gamma'') ++ GT) & (w'0, Gamma0 ++ Gamma'0));
+[ PPermut_simpl | apply ok_Bg_split4 with (w:=w0)]; rew_app; auto.
 assert ((w, Gamma) :: G & (w0, Gamma0) ~=~
   (G & (w, Gamma)) & (w0, Gamma0)) by auto;
 rewrite H4 in Ok_Bg; rewrite <- H2 in Ok_Bg; rew_app in *;
-remember (GH ++ (w, Gamma) :: GT) as GHT;
-assert (GH ++ (w, Gamma) :: GT ++ (w0, Gamma'0) :: (w'0, Gamma0) :: nil ~=~
-  GHT & (w0, Gamma'0) & (w'0, Gamma0)) by (subst; rew_app; auto);
+remember (GH ++ (w, Gamma'') :: GT) as GHT;
+assert (GH ++ (w, Gamma'') :: GT ++ (w0, Gamma'0) :: (w'0, Gamma0) :: nil ~=~
+  GHT & (w0, Gamma'0) & (w'0, Gamma0)) by (subst; rew_app; auto).
 rewrite H5; apply ok_Bg_swap_worlds; subst; rew_app in *; auto.
-eapply IHHT; auto.
+eapply IHHT; auto; PPermut_simpl.
 apply PPermut_last_rev_simpl with (a:=(w, Gamma)); rew_app in *;
-transitivity (GH ++ GT ++ (w0, Gamma0) :: (w'0, Gamma'0) :: (w, Gamma) :: nil);
-auto.
-rew_app; auto.
+rewrite H; rewrite H0; PPermut_simpl.
+transitivity (GH & (w, Gamma) ++ GT); PPermut_simpl.
 
 case_if.
 inversion H2; subst;
@@ -1260,179 +1298,194 @@ assert (G ~=~ G0 & (w'0, Gamma'0) /\ Gamma *=* Gamma'') by
   (apply ok_Bg_impl_ppermut with (w:=w''); [ | rewrite H; rewrite H0]; eauto);
 destruct H3; apply t_unbox_fetch_LF with (G:=G0) (Gamma := Gamma'0 ++ Gamma);
 [ rewrite H3 in Ok_Bg | apply IHHT | rewrite H1]; eauto.
+apply ok_Bg_split9 with (w':=w'');
+apply ok_Bg_ppermut with (G:= (w'', Gamma)::G0 & (w'0, Gamma'0) & (w0, Gamma0));
+eauto; PPermut_simpl.
+rewrite H3; PPermut_simpl.
 destruct (eq_var_dec w w'0).
 subst; assert (G ~=~ G0 & (w'', Gamma'') /\ Gamma *=* Gamma'0) by
-  (apply ok_Bg_impl_ppermut with (w:=w'0); [ | rewrite H; rewrite H0]; eauto);
+  (apply ok_Bg_impl_ppermut with (w:=w'0); [ | rewrite H; rewrite H0];
+   eauto; PPermut_simpl);
 destruct H3;
 apply t_unbox_fetch_LF with (G:=G0) (Gamma := Gamma ++ Gamma'');
 [ rewrite H3 in Ok_Bg |
   eapply IHHT with (G':=G0 & (w0, Gamma0)) (Gamma' := Gamma'') |
   rewrite H1]; eauto.
+eapply ok_Bg_split9; eauto.
+rewrite H3; PPermut_simpl.
 assert (G0 & (w'0, Gamma'0) & (w'', Gamma'')  ~=~ G & (w, Gamma)) by
   (symmetry; transitivity G'; auto);
-assert (exists GH, exists GT, G0 & (w'0, Gamma'0) = GH & (w, Gamma) ++ GT)
-  as Split by (apply PPermut_split_neq with (w:=w'')
-               (Gamma:=Gamma'') (G':= G); eauto);
-assert (exists GH, exists GT, G0 = GH & (w, Gamma) ++ GT) as Split' by
-  (destruct Split as (GH, Split); destruct Split as (GT);
+assert (exists Gamma'', exists GH, exists GT,
+  Gamma'' *=* Gamma /\ G0 & (w'0, Gamma'0) = GH & (w, Gamma'') ++ GT)
+  as Split.
+apply PPermut_split_neq with (w:=w'')
+  (Gamma:=Gamma'') (G':= G); auto; right; intro; subst; elim H2; auto.
+assert (exists Gamma'', exists GH, exists GT,
+  Gamma'' *=* Gamma /\ G0 = GH & (w, Gamma'') ++ GT) as Split' by
+  (destruct Split as (Gamma''', (GH, Split));
+    destruct Split as (GT, (Ha, Hb));
    apply PPermut_split_neq with (w:=w'0) (Gamma:=Gamma'0) (G':=GH ++ GT);
    [ rew_app; transitivity (GH & (w, Gamma) ++ GT) |
-     right; intro; subst; elim n]; auto; rewrite H4; auto);
-destruct Split' as (GH, Split'); destruct Split' as (GT);
+     right; intro; subst; elim n]; auto; rewrite Hb; auto);
+destruct Split' as (Gamma''',(GH, Split'));
+destruct Split' as (GT, (Ha, Hb));
 apply t_unbox_fetch_LF with (G:=GH++GT & (w'0, Gamma'0++Gamma''))
   (Gamma:=Gamma).
 apply ok_Bg_ppermut with (G':=(G' & (w0, Gamma0))) in Ok_Bg;
-[ | rewrite <- H; auto]; rewrite H0 in Ok_Bg; subst G0;
+[ | rewrite <- H; auto]; rewrite H0 in Ok_Bg; subst G0.
 apply ok_Bg_ppermut with
-  (G:= (GH & (w, Gamma) ++ GT) & (w'0, Gamma'0 ++ Gamma'') & (w0, Gamma0));
-[ rew_app | ]; auto || eauto.
+  (G:= (GH & (w, Gamma''') ++ GT) & (w'0, Gamma'0 ++ Gamma'') & (w0, Gamma0));
+[ rew_app | ]; auto; try PPermut_simpl; eapply ok_Bg_split6; eauto.
 eapply IHHT with (w1:=w) (Gamma1:=Gamma) (G0:=GH++GT & (w0,Gamma0))
   (Gamma':=Gamma'0) (Gamma'':=Gamma''); auto.
-assert (G & (w, Gamma) ~=~ G0 & (w'0, Gamma'0) & (w'', Gamma'')) by
-  (transitivity G'; auto);
-subst; rew_app in *;
-assert (G & (w, Gamma) ~=~
-       (GH ++ GT ++ (w'0, Gamma'0) :: (w'', Gamma'') :: nil) &  (w, Gamma)) by
- (transitivity (GH ++ (w, Gamma) :: GT ++  (w'0, Gamma'0) ::
-   (w'', Gamma'') :: nil); auto);
-transitivity ((GH ++ GT ++ (w'0, Gamma'0) :: (w'', Gamma'') :: nil) &
-  (w0, Gamma0)); [ | rew_app; auto];
-apply PPermut_last; auto; apply PPermut_last_rev_simpl with (a:=(w, Gamma));
-eauto; rew_app; auto.
-rew_app; auto.
-rew_app; symmetry;
-transitivity (G0 & (w'0, Gamma'0 ++ Gamma'')); auto;
-subst; rew_app; auto.
+PPermut_simpl. apply PPermut_last_rev_simpl with (a:=(w, Gamma));
+rewrite <- H3; subst; PPermut_simpl.
+PPermut_simpl.
+rewrite H1; subst; PPermut_simpl.
 
 (* here *)
 case_if.
 inversion H0; subst; rewrite H in Ok_Bg;
 apply ok_Bg_first_last_neq in Ok_Bg; elim Ok_Bg; auto.
 constructor;
-[ rewrite H in Ok_Bg | apply IHHT with (Gamma:=Gamma0)]; eauto.
+[ rewrite H in Ok_Bg | apply IHHT with (Gamma:=Gamma0)]; eauto;
+eapply ok_Bg_split2; eauto.
 
 case_if; constructor;
 [ rewrite H in Ok_Bg |
-  apply IHHT with (Gamma:=Gamma0) ]; eauto.
+  apply IHHT with (Gamma:=Gamma0) ]; eauto;
+eapply ok_Bg_split2; eauto.
 
 case_if.
 inversion H1; subst; rewrite H in Ok_Bg;
 apply ok_Bg_first_last_neq in Ok_Bg; elim Ok_Bg; auto.
-constructor; [rewrite H0; rewrite H in Ok_Bg | eapply IHHT]; eauto.
+constructor; [rewrite H0; rewrite H in Ok_Bg | eapply IHHT]; eauto;
+eapply ok_Bg_split3; eauto.
 
 (* get_here *)
 case_if.
-inversion H2; subst;
-assert (G ~=~ G'0 /\ Gamma *=* Gamma') as HP by
-  (apply ok_Bg_impl_ppermut with (w:=w');
+inversion H1; subst;
+assert (G ~=~ G'0 /\ Gamma *=* Gamma'0) as HP by
+  (apply ok_Bg_impl_ppermut with (w:=w'0);
    [eauto | rewrite H; rewrite H0; auto]);
 destruct HP; constructor.
-rewrite <- H3; apply ok_Bg_split2 with (w:=w');
+rewrite <- H2; apply ok_Bg_split2 with (w:=w'0);
 eapply ok_Bg_permut; eauto.
 apply ContextPermutImpl with (Gamma:=Gamma0 ++ Gamma);
 [ permut_simpl |
   apply IHHT] ; auto.
-assert (G'0 & (w', Gamma') ~=~ G & (w, Gamma)) by
+assert (G'0 & (w'0, Gamma'0) ~=~ G & (w, Gamma)) by
   (symmetry; transitivity G'; auto);
-assert (exists GH, exists GT, G'0 = GH & (w, Gamma) ++ GT) as Split by
+assert (exists Gamma'', exists GH, exists GT,
+  Gamma'' *=* Gamma /\ G'0 = GH & (w, Gamma'') ++ GT) as Split by
   (eapply PPermut_split_neq; eauto; right; intro; subst; elim H1; reflexivity);
-destruct Split as (GH, Split); destruct Split as (GT); subst;
+destruct Split as (Gamma'', (GH, Split)); destruct Split as (GT, H3);
+destruct H3 as (H3a, H3b).
 apply t_get_here_LF with (G:=GH++GT) (Gamma:=Gamma).
 assert ((w, Gamma) :: G & (w0, Gamma0) ~=~ G & (w, Gamma) & (w0, Gamma0)) by
-  auto;
-rewrite H4 in Ok_Bg; rewrite <- H3 in Ok_Bg; rew_app in *;
-assert (GH & (w, Gamma) ++ GT ~=~ (w, Gamma) :: GH ++ GT) by (symmetry; eauto);
+  auto.
+rewrite H3 in Ok_Bg; rewrite <- H2 in Ok_Bg; rew_app in *;
+assert (GH & (w, Gamma) ++ GT ~=~ (w, Gamma) :: GH ++ GT) by (PPermut_simpl);
 apply ok_Bg_ppermut with
-  (G:= (GH & (w, Gamma) ++ GT) & (w0, Gamma0 ++ Gamma'));
-[ rewrite H5 |
-  apply ok_Bg_split4 with (w:=w')]; rew_app; auto.
-eapply IHHT with (w1:=w) (Gamma1:=Gamma); auto.
-apply PPermut_last_rev_simpl with (a:=(w, Gamma)); rew_app in *; auto.
-rew_app; auto.
+  (G:= (GH & (w, Gamma) ++ GT) & (w0, Gamma0 ++ Gamma'0));
+[ rewrite H4 |
+  apply ok_Bg_split4 with (w:=w'0)]; rew_app; auto.
+subst; rew_app in *;
+apply ok_Bg_ppermut with
+  (G:=(GH ++ (w, Gamma'') :: GT ++ (w'0, Gamma'0) :: (w0, Gamma0) :: nil));
+try PPermut_simpl; auto.
+eapply IHHT with (w1:=w) (Gamma1:=Gamma); auto; subst; symmetry; PPermut_simpl;
+apply PPermut_last_rev_simpl with (a:=(w, Gamma)); rew_app in *; auto;
+rew_app; auto; rewrite <- H2; PPermut_simpl.
+apply PPermut_last_rev_simpl with (a:=(w, Gamma)); rew_app in *; auto; subst;
+PPermut_simpl.
 
 case_if;
-[ inversion H2; subst; apply ok_Bg_first_last_neq in Ok_Bg; elim Ok_Bg; auto |
-  destruct (eq_var_dec w w')].
-subst; assert (G ~=~ G'0 /\ Gamma *=* Gamma') by
-  (apply ok_Bg_impl_ppermut with (w:=w'); [ | rewrite <- H0]; eauto);
-destruct H3; constructor.
-rewrite <- H3; apply ok_Bg_permut with (Ctx := (Gamma ++ Gamma0)); eauto.
+[ inversion H1; subst; apply ok_Bg_first_last_neq in Ok_Bg; elim Ok_Bg; auto |
+  destruct (eq_var_dec w w'0)].
+subst; assert (G ~=~ G'0 /\ Gamma *=* Gamma'0) by
+  (apply ok_Bg_impl_ppermut with (w:=w'0); [ | rewrite <- H0]; eauto);
+destruct H2; constructor.
+rewrite <- H2; apply ok_Bg_permut with (Ctx := (Gamma ++ Gamma0)); eauto;
+eapply ok_Bg_split2; eauto.
 apply ContextPermutImpl with (Gamma:=Gamma ++ Gamma0);
 [ permut_simpl |
-  eapply IHHT with (w:=w') (Gamma1:=Gamma) (Gamma':=Gamma0)] ; auto.
-assert (G'0 & (w', Gamma') ~=~ G & (w, Gamma)) by
+  eapply IHHT with (w:=w'0) (Gamma1:=Gamma) (Gamma':=Gamma0)] ; auto.
+assert (G'0 & (w'0, Gamma'0) ~=~ G & (w, Gamma)) by
   (symmetry; transitivity G'; auto);
-assert (exists GH, exists GT, G'0 = GH & (w, Gamma) ++ GT) as Split by
+assert (exists Gamma'', exists GH, exists GT,
+  Gamma'' *=* Gamma /\ G'0 = GH & (w, Gamma'') ++ GT) as Split by
   (eapply PPermut_split_neq; eauto; right; intro; subst; elim H1; reflexivity);
-destruct Split as (GH, Split); destruct Split as (GT); subst;
+destruct Split as (Gamma'', (GH, Split));
+destruct Split as (GT, (Ha, Hb)); subst;
 apply t_get_here_LF with (G:=GH++GT) (Gamma:=Gamma).
-assert (GH & (w, Gamma) ++ GT ~=~ (w, Gamma) :: GH ++ GT) by (symmetry; eauto);
+assert (GH & (w, Gamma) ++ GT ~=~ (w, Gamma) :: GH ++ GT)
+  by PPermut_simpl;
 apply ok_Bg_ppermut with
-  (G:= (GH & (w, Gamma) ++ GT) & (w', Gamma0 ++ Gamma'));
-[ rewrite H4 | apply ok_Bg_split4 with (w:=w0)]; rew_app; auto;
+  (G:= (GH & (w, Gamma'') ++ GT) & (w'0, Gamma0 ++ Gamma'0));
+[ PPermut_simpl | apply ok_Bg_split4 with (w:=w0)]; rew_app; auto.
 assert ((w, Gamma) :: G & (w0, Gamma0) ~=~
   (G & (w, Gamma)) & (w0, Gamma0)) by auto;
-rewrite H5 in Ok_Bg; rewrite <- H3 in Ok_Bg; rew_app in *;
-remember (GH ++ (w, Gamma) :: GT) as GHT;
-assert (GH ++ (w, Gamma) :: GT ++ (w0, Gamma') :: (w', Gamma0) :: nil ~=~
-  GHT & (w0, Gamma') & (w', Gamma0)) by (subst; rew_app; auto);
-rewrite H6; apply ok_Bg_swap_worlds; subst; rew_app in *; auto.
-eapply IHHT; auto.
+rewrite H4 in Ok_Bg; rewrite <- H2 in Ok_Bg; rew_app in *;
+remember (GH ++ (w, Gamma'') :: GT) as GHT;
+assert (GH ++ (w, Gamma'') :: GT ++ (w0, Gamma'0) :: (w'0, Gamma0) :: nil ~=~
+  GHT & (w0, Gamma'0) & (w'0, Gamma0)) by (subst; rew_app; auto).
+rewrite H5; apply ok_Bg_swap_worlds; subst; rew_app in *; auto.
+eapply IHHT; auto; PPermut_simpl.
 apply PPermut_last_rev_simpl with (a:=(w, Gamma)); rew_app in *;
-transitivity (GH ++ GT ++ (w0, Gamma0) :: (w', Gamma') :: (w, Gamma) :: nil);
-auto.
-rew_app; auto.
+rewrite H; rewrite H0; PPermut_simpl.
+transitivity (GH & (w, Gamma) ++ GT); PPermut_simpl.
 
 case_if.
-inversion H3; subst;
-assert (G ~=~ G0 & (w', Gamma') /\ Gamma *=* Gamma'') by
-  (apply ok_Bg_impl_ppermut with (w:=w'');
-   [ | rewrite H; rewrite H0]; eauto);
-destruct H4; apply t_get_here_LF with (G:=G0) (Gamma := Gamma' ++ Gamma);
-[ rewrite H4 in Ok_Bg | apply IHHT | rewrite H1]; eauto.
-destruct (eq_var_dec w w').
-subst; assert (G ~=~ G0 & (w'', Gamma'') /\ Gamma *=* Gamma') by
-  (apply ok_Bg_impl_ppermut with (w:=w'); [ | rewrite H; rewrite H0]; eauto);
-destruct H4;
+inversion H2; subst;
+assert (G ~=~ G0 & (w'0, Gamma'0) /\ Gamma *=* Gamma'') by
+  (apply ok_Bg_impl_ppermut with (w:=w''); [ | rewrite H; rewrite H0]; eauto);
+destruct H3; apply t_get_here_LF with (G:=G0) (Gamma := Gamma'0 ++ Gamma);
+[ rewrite H3 in Ok_Bg | apply IHHT | rewrite H1]; eauto.
+apply ok_Bg_split9 with (w':=w'');
+apply ok_Bg_ppermut with (G:= (w'', Gamma)::G0 & (w'0, Gamma'0) & (w0, Gamma0));
+eauto; PPermut_simpl.
+rewrite H3; PPermut_simpl.
+destruct (eq_var_dec w w'0).
+subst; assert (G ~=~ G0 & (w'', Gamma'') /\ Gamma *=* Gamma'0) by
+  (apply ok_Bg_impl_ppermut with (w:=w'0); [ | rewrite H; rewrite H0];
+   eauto; PPermut_simpl);
+destruct H3;
 apply t_get_here_LF with (G:=G0) (Gamma := Gamma ++ Gamma'');
-[ rewrite H4 in Ok_Bg |
+[ rewrite H3 in Ok_Bg |
   eapply IHHT with (G':=G0 & (w0, Gamma0)) (Gamma' := Gamma'') |
   rewrite H1]; eauto.
-assert (G0 & (w', Gamma') & (w'', Gamma'')  ~=~ G & (w, Gamma)) by
+eapply ok_Bg_split9; eauto.
+rewrite H3; PPermut_simpl.
+assert (G0 & (w'0, Gamma'0) & (w'', Gamma'')  ~=~ G & (w, Gamma)) by
   (symmetry; transitivity G'; auto);
-assert (exists GH, exists GT, G0 & (w', Gamma') = GH & (w, Gamma) ++ GT)
-  as Split by (apply PPermut_split_neq with (w:=w'')
-               (Gamma:=Gamma'') (G':= G); eauto);
-assert (exists GH, exists GT, G0 = GH & (w, Gamma) ++ GT) as Split' by
-  (destruct Split as (GH, Split); destruct Split as (GT);
-   apply PPermut_split_neq with (w:=w') (Gamma:=Gamma') (G':=GH ++ GT);
+assert (exists Gamma'', exists GH, exists GT,
+  Gamma'' *=* Gamma /\ G0 & (w'0, Gamma'0) = GH & (w, Gamma'') ++ GT)
+  as Split.
+apply PPermut_split_neq with (w:=w'')
+  (Gamma:=Gamma'') (G':= G); auto; right; intro; subst; elim H2; auto.
+assert (exists Gamma'', exists GH, exists GT,
+  Gamma'' *=* Gamma /\ G0 = GH & (w, Gamma'') ++ GT) as Split' by
+  (destruct Split as (Gamma''', (GH, Split));
+    destruct Split as (GT, (Ha, Hb));
+   apply PPermut_split_neq with (w:=w'0) (Gamma:=Gamma'0) (G':=GH ++ GT);
    [ rew_app; transitivity (GH & (w, Gamma) ++ GT) |
-     right; intro; subst; elim n]; auto; rewrite H5; auto);
-destruct Split' as (GH, Split'); destruct Split' as (GT);
-apply t_get_here_LF with (G:=GH++GT & (w', Gamma'++Gamma''))
+     right; intro; subst; elim n]; auto; rewrite Hb; auto);
+destruct Split' as (Gamma''',(GH, Split'));
+destruct Split' as (GT, (Ha, Hb));
+apply t_get_here_LF with (G:=GH++GT & (w'0, Gamma'0++Gamma''))
   (Gamma:=Gamma).
 apply ok_Bg_ppermut with (G':=(G' & (w0, Gamma0))) in Ok_Bg;
-[ | rewrite <- H; auto]; rewrite H0 in Ok_Bg; subst G0;
+[ | rewrite <- H; auto]; rewrite H0 in Ok_Bg; subst G0.
 apply ok_Bg_ppermut with
-  (G:= (GH & (w, Gamma) ++ GT) & (w', Gamma' ++ Gamma'') & (w0, Gamma0));
-[ rew_app | ]; auto || eauto.
+  (G:= (GH & (w, Gamma''') ++ GT) & (w'0, Gamma'0 ++ Gamma'') & (w0, Gamma0));
+[ rew_app | ]; auto; try PPermut_simpl; eapply ok_Bg_split6; eauto.
 eapply IHHT with (w1:=w) (Gamma1:=Gamma) (G0:=GH++GT & (w0,Gamma0))
-  (Gamma':=Gamma') (Gamma'':=Gamma''); auto.
-assert (G & (w, Gamma) ~=~ G0 & (w', Gamma') & (w'', Gamma'')) by
-  (transitivity G'; auto);
-subst; rew_app in *;
-assert (G & (w, Gamma) ~=~
-       (GH ++ GT ++ (w', Gamma') :: (w'', Gamma'') :: nil) &  (w, Gamma)) by
- (transitivity (GH ++ (w, Gamma) :: GT ++  (w', Gamma') ::
-   (w'', Gamma'') :: nil); auto);
-transitivity ((GH ++ GT ++ (w', Gamma') :: (w'', Gamma'') :: nil) &
-  (w0, Gamma0)); [ | rew_app; auto];
-apply PPermut_last; auto; apply PPermut_last_rev_simpl with (a:=(w, Gamma));
-eauto; rew_app; auto.
-rew_app; auto.
-rew_app; symmetry;
-transitivity (G0 & (w', Gamma' ++ Gamma'')); auto;
-subst; rew_app; auto.
+  (Gamma':=Gamma'0) (Gamma'':=Gamma''); auto.
+PPermut_simpl. apply PPermut_last_rev_simpl with (a:=(w, Gamma));
+rewrite <- H3; subst; PPermut_simpl.
+PPermut_simpl.
+rewrite H1; subst; PPermut_simpl.
 
 (* letdia *)
 case_if.
@@ -1440,38 +1493,44 @@ inversion H1; subst; rewrite H0 in Ok_Bg;
 apply ok_Bg_first_last_neq in Ok_Bg; elim Ok_Bg; auto.
 apply t_letdia_LF with (L_w:=L_w \u \{w'}) (L_t:=L_t) (A:=A);
 [ rewrite H0 in Ok_Bg |
-  eapply IHHT with (w:=w0) (Gamma:=Gamma0) | ]; eauto;
+  eapply IHHT with (w:=w0) (Gamma:=Gamma0) | ]; eauto.
+eapply ok_Bg_split2; eauto.
 intros; rewrite notin_union in H3; destruct H3;
 rewrite notin_singleton in H4;
-unfold open_var in *; unfold open_ctx in *;
+unfold open_t in *; unfold open_w in *;
 rewrite <- subst_w_comm; auto;
 rewrite subst_order_irrelevant_free;
-[ eapply H with (w:=w0) (Gamma:=Gamma0) (w':=w'0) | simpl]; eauto.
+[ eapply H with (w:=w0) (Gamma:=Gamma0) (w':=w'0) | simpl]; eauto;
+rewrite H0; PPermut_simpl.
 
 case_if.
 apply t_letdia_LF with (L_w:=L_w \u \{w0}) (L_t:=L_t) (A:=A);
-[ rewrite H0 in Ok_Bg | eapply IHHT with (w:=w0) (Gamma:=Gamma0) | ]; eauto;
+[ rewrite H0 in Ok_Bg | eapply IHHT with (w:=w0) (Gamma:=Gamma0) | ]; eauto.
+eapply ok_Bg_split2; eauto.
 intros; rewrite notin_union in H2; destruct H2;
 rewrite notin_singleton in H3;
-unfold open_var in *; unfold open_ctx in *;
+unfold open_t in *; unfold open_w in *;
 rewrite <- subst_w_comm; auto;
 rewrite subst_order_irrelevant_free;
-[ eapply H with (w:=w0) (Gamma:=Gamma0) (w':=w'0) | simpl]; eauto.
+[ eapply H with (w:=w0) (Gamma:=Gamma0) (w':=w'0) | simpl]; eauto;
+rewrite H0; PPermut_simpl.
 
 case_if.
 inversion H2; subst; rewrite H0 in Ok_Bg;
 apply ok_Bg_first_last_neq in Ok_Bg; elim Ok_Bg; auto.
 apply t_letdia_LF with (L_w:=L_w \u \{w''}) (L_t:=L_t) (A:=A);
 [ rewrite H0 in Ok_Bg; rewrite H1 |
-  eapply IHHT with (w:=w0) (Gamma:=Gamma0) | ]; eauto;
+  eapply IHHT with (w:=w0) (Gamma:=Gamma0) | ]; eauto.
+eapply ok_Bg_split3; eauto.
 intros; rewrite notin_union in H4; destruct H4;
 rewrite notin_singleton in H5;
-unfold open_var in *; unfold open_ctx in *;
+unfold open_t in *; unfold open_w in *;
 rewrite <- subst_w_comm; auto;
 rewrite subst_order_irrelevant_free; simpl; auto;
 eapply H with (w:=w0) (Gamma:=Gamma0) (G0:=G0 & ((w'0, (v', A)::nil)))
   (Gamma':=Gamma') (Gamma'':=Gamma''); auto;
-[ rewrite H0 |rewrite H1 ]; rew_app; auto.
+[ rewrite H0 |rewrite H1 ]; rew_app; auto;
+PPermut_simpl.
 
 (* letdia_get *)
 case_if.
@@ -1480,12 +1539,13 @@ assert (G ~=~ G' /\ Gamma *=* Gamma') by
   (apply ok_Bg_impl_ppermut with (w:=w'); [ | transitivity G0]; eauto);
 destruct H4;
 eapply t_letdia_LF with (L_w := L_w \u \{w'}).
-rewrite <- H4; apply ok_Bg_permut with (Ctx:=(Gamma0 ++ Gamma)); auto || eauto.
+rewrite <- H4; apply ok_Bg_permut with (Ctx:=(Gamma0 ++ Gamma)); auto;
+eapply ok_Bg_split1; eauto.
 apply ContextPermutImpl with (Gamma := Gamma0++Gamma); [permut_simpl|]; auto;
 eapply IHHT; auto.
 intros; rewrite notin_union in H7; destruct H7;
 rewrite notin_singleton in H8;
-unfold open_var in *; unfold open_ctx in *;
+unfold open_t in *; unfold open_w in *;
 rewrite <- subst_w_comm; auto;
 rewrite subst_order_irrelevant_free; simpl; auto;
 eapply H with (v':=v') (w'0:=w'0) (w:=w0); auto;
@@ -1494,89 +1554,86 @@ destruct (eq_var_dec w w0).
 subst; apply ok_Bg_first_last_neq in Ok_Bg; elim Ok_Bg; auto.
 assert (G' & (w', Gamma') ~=~ G & (w, Gamma)) by
   (symmetry; transitivity G0; auto);
-assert (exists GH, exists GT, G' = GH & (w, Gamma) ++ GT) by
-  (eapply PPermut_split_neq; eauto);
-destruct H5 as (GH, H5); destruct H5 as (GT, H5);
+assert (exists Gamma'', exists GH, exists GT,
+  Gamma'' *=* Gamma /\ G' = GH & (w, Gamma'') ++ GT) by
+  (eapply PPermut_split_neq; eauto; right; intro; subst; eauto);
+destruct H5 as (Gamma'', (GH, (GT, (Ha, Hb))));
 assert (G & (w, Gamma) ~=~
        (GH ++ GT ++ (w', Gamma') :: nil) &  (w, Gamma));
 [subst; symmetry | rew_app]; auto.
-apply PPermut_last; auto;
-apply PPermut_last_rev_simpl with (a:=(w, Gamma)); auto;
-transitivity ((GH & (w, Gamma) ++ GT) & (w', Gamma'));
-[rew_app in *; symmetry | ]; auto.
+rewrite <- H4; PPermut_simpl.
 apply t_letdia_get_LF with (L_w:=L_w \u \{w'}) (L_t:=L_t) (A:=A)
   (G:=GH++GT) (Gamma:=Gamma);
 assert ((w, Gamma) :: G & (w0, Gamma0) ~=~
   (GH ++ GT & (w', Gamma')) & (w, Gamma) & (w0, Gamma0)) by
-(rewrite <- H6; auto);
-rewrite H7 in Ok_Bg.
+  (PPermut_simpl; apply PPermut_last_rev_simpl with (a:=(w,Gamma)); auto).
+rewrite H6 in Ok_Bg.
 apply ok_Bg_ppermut with (G:=(GH ++ GT & (w, Gamma)) & (w0, Gamma0 ++ Gamma')).
-transitivity (((w, Gamma)::(GH++GT)) & (w0, Gamma0++Gamma'));
-[ | rew_app in *]; eauto.
-rew_app in *; eauto.
+PPermut_simpl.
+rew_app in *; eauto. eapply ok_Bg_split8; eauto.
 eapply IHHT with (w1:=w) (G0:=GH++GT) (w':=w0)
   (Gamma':=Gamma0) (Gamma'':=Gamma');
 auto.
-transitivity ((GH ++ GT & (w', Gamma')) & (w0, Gamma0));
-[ apply PPermut_last; auto;
-  apply PPermut_last_rev_simpl with (a:=(w, Gamma)) |
-  rew_app]; auto.
-intros; rewrite notin_union in H9; destruct H9;
-rewrite notin_singleton in H10;
-unfold open_var in *; unfold open_ctx in *;
+PPermut_simpl; apply PPermut_last_rev_simpl with (a:=(w, Gamma));
+rewrite H5; PPermut_simpl.
+intros; rewrite notin_union in H8; destruct H8;
+rewrite notin_singleton in H9;
+unfold open_t in *; unfold open_w in *;
 rewrite <- subst_w_comm; auto;
 rewrite subst_order_irrelevant_free; simpl; auto;
 eapply H with (w1:=w0) (Gamma1:=Gamma0); auto.
-rew_app; constructor; auto.
-transitivity ((GH ++ GT & (w', Gamma')) & (w, Gamma)); [ | rew_app]; auto.
-subst; rew_app; auto.
+rewrite H5; PPermut_simpl.
+subst; PPermut_simpl.
 
 case_if.
 inversion H3; subst;
 apply ok_Bg_first_last_neq in Ok_Bg; elim Ok_Bg; auto.
 destruct (eq_var_dec w w').
-subst; assert (G ~=~ G' /\ Gamma *=* Gamma') by
-( apply ok_Bg_impl_ppermut with (w:=w'); eauto);
+subst; assert (G ~=~ G' /\ Gamma *=* Gamma').
+  apply ok_Bg_impl_ppermut with (w:=w'); auto. eauto with ok_bg_rew.
+  transitivity G0; auto.
 destruct H4;
 apply t_letdia_LF with (L_w:=L_w \u \{w0}) (L_t:=L_t) (A:=A).
-rewrite <- H4; apply ok_Bg_permut with (Ctx := Gamma ++ Gamma0); auto || eauto.
+rewrite <- H4; apply ok_Bg_permut with (Ctx := Gamma ++ Gamma0); auto;
+eapply ok_Bg_split2; eauto.
 apply ContextPermutImpl with (Gamma:=Gamma++Gamma0); auto;
 eapply IHHT with (Gamma1:=Gamma); eauto.
 intros; rewrite <- H4;
 apply ContextPermutImpl with (Gamma:=Gamma++Gamma0); auto;
-unfold open_var in *; unfold open_ctx in *;
+unfold open_t in *; unfold open_w in *;
 rewrite <- subst_w_comm; auto;
-rewrite subst_order_irrelevant_free; simpl; auto;
+rewrite subst_order_irrelevant_free; simpl; auto.
 eapply H with (w'0 := w'0); eauto.
 assert (G' & (w', Gamma') ~=~ G & (w, Gamma)) by
   (symmetry; transitivity G0; auto);
-assert (exists GH, exists GT, G' = GH & (w, Gamma) ++ GT) by
-  (eapply PPermut_split_neq; eauto);
-destruct H5 as (GH, H5); destruct H5 as (GT, H5);
+assert (exists Gamma'', exists GH, exists GT,
+  Gamma'' *=* Gamma /\ G' = GH & (w, Gamma'') ++ GT) by
+  (eapply PPermut_split_neq; eauto).
+destruct H5 as (Gamma'', (GH, (GT, (Ha, Hb)))).
 apply t_letdia_get_LF with (L_w:=L_w \u \{w0})
   (L_t:=L_t) (A:=A) (G:=GH++GT) (Gamma:=Gamma).
 subst; assert ((w, Gamma) :: G & (w0, Gamma0) ~=~
-  (GH & (w, Gamma) ++ GT) & (w', Gamma') & (w0, Gamma0)) by (rewrite H4; auto);
-rewrite H5 in Ok_Bg;
-apply ok_Bg_ppermut with (G:= GH & (w, Gamma) ++ GT & (w', Gamma' ++ Gamma0));
-rew_app in *; [ auto | ];
-apply ok_Bg_ppermut with (G:=(GH ++ (w, Gamma) :: GT) & (w', Gamma' ++ Gamma0));
+  (GH & (w, Gamma'') ++ GT) & (w', Gamma') & (w0, Gamma0)) by
+(rewrite H4; auto).
+rewrite H5 in Ok_Bg.
+apply ok_Bg_ppermut with (G:= GH & (w, Gamma'') ++ GT & (w', Gamma' ++ Gamma0));
+rew_app in *; [ PPermut_simpl | ];
+apply ok_Bg_ppermut with
+  (G:=(GH ++ (w, Gamma'') :: GT) & (w', Gamma' ++ Gamma0));
 [ | apply ok_Bg_split4 with (w:=w0)]; rew_app; auto;
-apply ok_Bg_ppermut with (G:=GH ++ (w, Gamma) :: GT ++ (w', Gamma') ::
+apply ok_Bg_ppermut with (G:=GH ++ (w, Gamma'') :: GT ++ (w', Gamma') ::
   (w0, Gamma0) :: nil); eauto.
-eapply IHHT; auto;
-apply PPermut_last; auto; apply PPermut_last_rev_simpl with (a:=(w, Gamma));
-transitivity (GH & (w, Gamma) ++ GT & (w', Gamma')); [ | rew_app]; auto;
-subst; symmetry; rew_app in *; auto.
-intros; rewrite notin_union in H7; destruct H7;
-rewrite notin_singleton in H8; unfold open_var in *; unfold open_ctx in *;
+eapply IHHT; auto.
+PPermut_simpl; apply PPermut_last_rev_simpl with (a:=(w, Gamma));
+rewrite <- H4; subst; PPermut_simpl.
+intros. rewrite notin_union in H6; destruct H6;
+rewrite notin_singleton in H7; unfold open_t in *; unfold open_w in *;
 rewrite <- subst_w_comm; auto;
 rewrite subst_order_irrelevant_free; simpl; auto;
-eapply H with (w1:=w0) (Gamma1:=Gamma0); auto;
-rew_app; constructor; auto;
-subst; rew_app in *; symmetry;
-transitivity ( GH ++ (w, Gamma) :: GT & (w', Gamma')); auto.
-subst; symmetry; auto.
+eapply H with (w1:=w0) (Gamma1:=Gamma0); auto; PPermut_simpl.
+apply PPermut_last_rev_simpl with (a:=(w,Gamma));
+rewrite <- H4; subst; PPermut_simpl.
+subst; PPermut_simpl.
 
 case_if.
 inversion H4; subst;
@@ -1586,24 +1643,32 @@ assert (G ~=~ G1 & (w', Gamma') /\ Gamma *=* Gamma'') by
 destruct H5;
 eapply t_letdia_get_LF with (G:=G1) (Gamma:=Gamma'++Gamma) (L_w:=L_w \u \{w''}).
 rewrite H5 in Ok_Bg; eauto.
-eapply IHHT with (Gamma':=Gamma'); auto.
-intros; unfold open_var in *; unfold open_ctx in *;
+clear H HT2 IHHT.
+eapply ok_Bg_split2; eauto; apply ok_Bg_ppermut with
+  (G:=(w'', Gamma) :: G1 & (w', Gamma') & (w0, Gamma0));
+eauto; PPermut_simpl.
+eapply IHHT with (Gamma':=Gamma'); auto;
+try PPermut_simpl.
+intros; unfold open_t in *; unfold open_w in *;
 rewrite <- subst_w_comm; auto;
 rewrite subst_order_irrelevant_free; simpl; auto;
 eapply H with (w:=w0) (G0:=(w'0, (v',A)::nil)::G1)
   (Gamma':=Gamma') (Gamma'':=Gamma); auto;
 [ eauto | rew_app]; constructor; [ | symmetry]; auto;
 rewrite H5; rew_app; auto.
-symmetry; transitivity (G1 & (w', Gamma' ++ Gamma'')); auto.
-destruct (eq_var_dec w w'); subst.
-assert (G ~=~ G1 & (w'', Gamma'') /\ Gamma *=* Gamma') by
-  (apply ok_Bg_impl_ppermut with (w:=w'); [ | transitivity G0]; eauto);
+rewrite H2; PPermut_simpl.
+destruct (eq_var_dec w w').
+subst.
+assert (G ~=~ G1 & (w'', Gamma'') /\ Gamma *=* Gamma').
+  apply ok_Bg_impl_ppermut with (w:=w'); [ | transitivity G0]; eauto;
+  rewrite H1; PPermut_simpl.
 destruct H5;
 eapply t_letdia_get_LF with (G:=G1) (Gamma:=Gamma++Gamma'')
   (L_w:=L_w \u \{w''}) (L_t := L_t).
-rewrite H5 in Ok_Bg; eauto.
-eapply IHHT with (w:=w'); auto.
-intros; unfold open_var in *; unfold open_ctx in *;
+clear H HT2 IHHT.
+rewrite H5 in Ok_Bg; eapply ok_Bg_split9; eauto.
+eapply IHHT with (w:=w'); auto; PPermut_simpl.
+intros; unfold open_t in *; unfold open_w in *;
 rewrite <- subst_w_comm; auto;
 rewrite subst_order_irrelevant_free; simpl; auto;
 eapply H with (w:=w0) (G0:=(w'0, (v',A)::nil)::G1)
@@ -1611,48 +1676,48 @@ eapply H with (w:=w0) (G0:=(w'0, (v',A)::nil)::G1)
 rew_app; constructor; auto;
 symmetry; transitivity ((G1 ++ (w'', Gamma'')::nil) & (w', Gamma)); auto;
 rew_app; auto.
-symmetry; transitivity (G1 & (w', Gamma' ++ Gamma'')); auto.
+rewrite H2; PPermut_simpl.
 assert (G & (w, Gamma) ~=~ G1 & (w', Gamma') & (w'', Gamma'')) by
   (symmetry; transitivity G0; symmetry; auto);
-assert (exists GH, exists GT, G1 & (w'', Gamma'') = GH & (w, Gamma) ++ GT) by
+assert (exists Gamma0, exists GH, exists GT,
+  Gamma0 *=* Gamma /\ G1 & (w'', Gamma'') = GH & (w, Gamma0) ++ GT) by
   (apply PPermut_split_neq with (w:=w') (G':=G) (Gamma:=Gamma');
-   try symmetry; auto; transitivity (G1 & (w', Gamma') & (w'', Gamma'')); auto);
-assert (exists GH, exists GT, G1 = GH & (w, Gamma) ++ GT) by
-  (destruct H6 as (GH, H6); destruct H6 as (GT, H6); subst;
+   try symmetry; auto; transitivity (G1 & (w', Gamma') & (w'', Gamma'')); auto;
+  PPermut_simpl).
+assert (exists Gamma0, exists GH, exists GT,
+  Gamma0 *=* Gamma /\ G1 = GH & (w, Gamma0) ++ GT) by
+  (destruct H6 as (Gamma5, (GH, (GT, (H6a, H6b)))); subst;
    apply PPermut_split_neq with (w:=w'') (G':=GH++GT) (Gamma:=Gamma''); auto;
-   [rewrite H6; rew_app; auto | right; intro; subst; elim H4; reflexivity]);
-destruct H7 as (GH, H7); destruct H7 as (GT, H7); subst;
+   [rewrite H6b; rew_app; auto | right; intro; subst; elim H4; reflexivity];
+  PPermut_simpl).
+destruct H7 as (Gamma'1, (GH, (GT, (H7a, H7b)))); subst.
 apply t_letdia_get_LF with (L_w:=L_w \u \{w''})
   (L_t:=L_t) (A:=A) (G:=GH++GT & (w', Gamma'++Gamma'')) (Gamma:=Gamma).
 assert ((w, Gamma) :: G & (w0, Gamma0) ~=~ G0  & (w0, Gamma0)) by
   (rewrite <- H0; auto);
-rewrite H7 in Ok_Bg; rewrite H1 in Ok_Bg;
-apply ok_Bg_ppermut with (G:= (GH & (w, Gamma) ++ GT) &
+rewrite H7 in Ok_Bg; rewrite H1 in Ok_Bg.
+apply ok_Bg_ppermut with (G:= (GH & (w, Gamma'1) ++ GT) &
   (w', Gamma' ++ Gamma'') & (w0, Gamma0));
-rew_app in *; eauto.
+rew_app in *; eauto; try PPermut_simpl.
+clear IHHT H HT2. eapply ok_Bg_split10; eauto.
 eapply IHHT with (w1:=w) (G0:=GH++GT & (w0, Gamma0))
   (Gamma':=Gamma') (Gamma'':=Gamma''); rew_app; auto;
 rew_app in *; transitivity ((GH ++ GT ++ (w', Gamma') ::
   (w'', Gamma'') :: nil) & (w0, Gamma0));
-[ apply PPermut_last | rew_app]; auto;
+[ PPermut_simpl | rew_app]; auto;
 apply PPermut_last_rev_simpl with (a:=(w, Gamma));
 rewrite H5; symmetry; transitivity (GH ++ GT ++ (w, Gamma) :: (w', Gamma') ::
-  (w'', Gamma'') :: nil); [rew_app |  apply PPermut_app_head; symmetry]; auto.
-intros; unfold open_var in *; unfold open_ctx in *;
+  (w'', Gamma'') :: nil); [rew_app |  apply PPermut_app_head; symmetry]; auto;
+try PPermut_simpl.
+intros; unfold open_t in *; unfold open_w in *;
 rewrite <- subst_w_comm; auto;
 rewrite subst_order_irrelevant_free; simpl; auto;
 eapply H with (G0:=(w'0, (v', A) :: nil) :: (GH ++ GT) & (w, Gamma))
-  (Gamma':=Gamma') (Gamma'':=Gamma''); auto.
-rew_app in *; constructor; auto;
-transitivity (GH ++ (w, Gamma) :: GT ++ (w', Gamma') :: (w'', Gamma'') :: nil);
-auto; rew_app in *; constructor; auto.
-rew_app in *; constructor; auto;
-transitivity (GH ++ (w, Gamma) :: GT ++ (w', Gamma') :: (w'', Gamma'') :: nil);
-auto; rew_app in *; constructor; auto.
-rew_app; symmetry;
-transitivity ((GH & (w, Gamma) ++ GT) & (w', Gamma'++ Gamma''));
-[ | rew_app]; auto.
-Admitted. (* "No more subgoals but non-instantiated existential variables" *)
+  (Gamma':=Gamma') (Gamma'':=Gamma''); auto; PPermut_simpl.
+apply PPermut_last_rev_simpl with (a:=(w, Gamma)); rewrite H5;
+PPermut_simpl.
+rewrite H2; PPermut_simpl.
+Admitted. (* No more subgoals but non-instantiated existential variables: 6 *)
 
 Lemma rename_w_preserv_types_new:
 forall G w Gamma A M G' w' Gamma'
@@ -1711,18 +1776,17 @@ right; inversion HT; subst;
 inversion H_lc_t; subst;
 inversion H_lc_w; subst;
 edestruct IHM1 with (A := A0 ---> A); eauto;
-[ inversion H0; subst; inversion HT1; subst |
-  destruct H0];
+[ inversion H0; subst; inversion HT1; subst; inversion H3 |
+  inversion H0];
 eexists; constructor; eauto;
-inversion H4; subst; auto;
-erewrite closed_ctx_subst_var; eauto; constructor.
+inversion H5; subst; auto.
 (* unbox & unbox_fetch *)
 right; inversion HT; subst;
 inversion H_lc_w; subst;
 inversion H_lc_t; subst.
 (* unbox *)
 edestruct IHM with (A := [*]A); eauto;
-[ inversion H0; subst; inversion HT0; subst |
+[ inversion H0; subst; inversion HT0; subst; inversion H3 |
   destruct H0];
 eexists; constructor; eauto;
 inversion H1; inversion H2; subst; auto;
@@ -1742,8 +1806,8 @@ assert (emptyEquiv (G0 & (w, nil)) = G0 & (w, nil)) by
    apply emptyEquiv_permut_split_last in H6; rewrite H6; reflexivity);
 rewrite H0; auto.
 inversion H0; subst; inversion HT0; subst;
-eexists; constructor; eauto; inversion H2; auto;
-erewrite closed_var_subst_ctx; eauto; constructor.
+eexists; constructor; eauto; inversion H2; auto; subst.
+inversion H3; subst; auto.
 destruct H0; eexists; constructor; eauto.
 (* here & get_here *)
 inversion HT; subst;
@@ -1757,11 +1821,16 @@ eauto using step_LF.
 (* get_here *)
 assert (Gamma = nil) by
   ( apply emptyEquiv_permut_empty with
-    (G:= (G0 & (w0, Gamma))) (G':=G) (w:=w0); auto; apply Mem_last);
-subst; edestruct IHM with (A := A0) (G := G0 & (w, nil)) (w:=w0); eauto;
+    (G:= (G0 & (w0, Gamma))) (G':=G) (w:=w0); auto;
+    apply Mem_last); subst;
+destruct IHM with (A := A0)
+                  (Ctx := (w0, (@nil ty)))
+                  (G := G0 & (w, nil))
+                  (w := w0);
+eauto.
 assert (emptyEquiv (G0 & (w, nil)) = G0 & (w, nil)) by
-  (repeat rewrite emptyEquiv_rewrite; simpl;
-   apply emptyEquiv_permut_split_last in H5; rewrite H5; reflexivity).
+  ( repeat rewrite emptyEquiv_rewrite; simpl;
+   apply emptyEquiv_permut_split_last in H6; rewrite H6; reflexivity);
 rewrite H0; auto.
 left; inversion H0; subst; inversion HT0; subst;
 econstructor; eauto using step_LF.
@@ -1775,9 +1844,11 @@ inversion H_lc_t; subst.
 edestruct IHM1 with (A := <*>A0); eauto;
 [ inversion H0; subst; inversion HT1; subst |
   destruct H0];
-eexists; constructor; eauto;
-try apply closed_t_succ; auto;
-inversion H5; inversion H8; subst; auto.
+eexists; constructor; eauto.
+inversion H5; subst; auto.
+inversion H7; subst; auto.
+inversion H5; subst; auto.
+inversion H7; subst; auto.
 (* letdia_get *)
 assert (Gamma = nil) by
   ( apply emptyEquiv_permut_empty with (G:= (G0 & (w0, Gamma))) (G':=G) (w:=w0);
@@ -1793,7 +1864,7 @@ rewrite H0; auto.
 inversion H0; subst; inversion HT1; subst;
 eexists; constructor; eauto;
 try apply closed_t_succ; auto;
-inversion H5; inversion H9; subst; auto.
+inversion H5; inversion H8; subst; auto.
 destruct H0;
 eexists; constructor; eauto;
 try apply closed_t_succ; auto;
@@ -1827,18 +1898,18 @@ try (inversion HeqCtx; subst);
 try (econstructor; eauto).
 (* appl_lam *)
 inversion HT1; subst;
-unfold open_var in *;
+unfold open_t in *;
 assert (exists v, v \notin L \u free_vars_LF M0) as HF by apply Fresh;
-destruct HF as (v_fresh);
+destruct HF as (v_fresh).
 rewrite subst_t_neutral_free with (v:=v_fresh);
-[ eapply subst_t_preserv_types_inner; eauto;
-  rewrite <- double_emptyEquiv |
+[ eapply subst_t_preserv_types_inner; eauto |
   rewrite notin_union in H; destruct H]; auto.
+rewrite <- double_emptyEquiv; auto.
 (* unbox_box *)
 inversion HT; subst;
 assert (exists v, v \notin L \u (free_worlds_LF M0)) as HF by apply Fresh;
 destruct HF as (w_fresh);
-unfold open_ctx in *;
+unfold open_w in *;
 replace ({{fwo w0 // bwo 0}}M0)
   with ({{fwo w0 // fwo w_fresh}} {{fwo w_fresh // bwo 0}}M0)
   by (rewrite subst_w_neutral_free; auto);
@@ -1849,13 +1920,13 @@ auto.
 inversion HT; subst;
 assert (exists v, v \notin L \u (free_worlds_LF M0)) as HF by apply Fresh;
 destruct HF as (w_fresh);
-unfold open_ctx in *;
+unfold open_w in *;
 replace ({{fwo w0 // bwo 0}}M0)
   with ({{fwo w0 // fwo w_fresh}} {{fwo w_fresh // bwo 0}}M0)
   by (rewrite subst_w_neutral_free; auto);
 replace (@nil (var * ty)) with (nil ++ (@nil (var * ty))); eauto;
 apply rename_w_preserv_types_old with (G := G & (w0, nil) & (w, Gamma));
-auto.
+auto; PPermut_simpl.
 (* unbox_fetch *)
 assert (Gamma = nil) by
   ( apply emptyEquiv_permut_empty with (G:= (G & (w, Gamma))) (G':=G0) (w:=w);
@@ -1877,7 +1948,7 @@ destruct HF as (w_fresh); destruct HF2 as (v_fresh);
 inversion HT; subst.
 (* letdia #1 *)
 rewrite notin_union in *; destruct H0; destruct H1;
-unfold open_var in *; unfold open_ctx in *;
+unfold open_t in *; unfold open_w in *;
 rewrite subst_t_neutral_free with (v:=v_fresh);
 [ rewrite subst_order_irrelevant_bound |
   apply subst_world_preserv_free_vars]; auto;
@@ -1890,10 +1961,10 @@ replace ((v_fresh, A) :: nil) with (nil ++ (v_fresh, A) :: nil) by auto;
 apply rename_w_preserv_types_new with
   (G:= (w_fresh, (v_fresh, A)::nil) :: emptyEquiv G0);
 [ rewrite <- subst_order_irrelevant_bound |
-  rew_app]; auto; constructor.
+  rew_app]; auto; try PPermut_simpl; constructor.
 (* letdia #2 *)
 rewrite notin_union in *; destruct H0; destruct H1;
-unfold open_var in *; unfold open_ctx in *;
+unfold open_t in *; unfold open_w in *;
 rewrite subst_t_neutral_free with (v:=v_fresh);
 [ rewrite subst_order_irrelevant_bound |
   apply subst_world_preserv_free_vars]; auto;
@@ -1905,19 +1976,20 @@ rewrite subst_t_neutral_free with (v:=v_fresh);
 rew_app;
 assert ( emptyEquiv (G & (w0, nil)) = G & (w0, nil)) by
    ( repeat rewrite emptyEquiv_rewrite; simpl;
-     apply emptyEquiv_permut_split_last in H7; rewrite H7; reflexivity);
+     apply emptyEquiv_permut_split_last in H5; rewrite H5; reflexivity);
 assert (Gamma = nil) by
   ( apply emptyEquiv_permut_empty with (G:= (G & (w, Gamma)))
     (G':=G0) (w:=w); auto; apply Mem_last);
 subst;
-rewrite <- H5 in HT0; auto.
+rewrite <- H7 in HT0; auto.
 apply rename_w_preserv_types_outer with (G0:=G) (Gamma'':=(v_fresh,A) :: nil)
-      (Gamma':=Gamma) (G:=G & (w, Gamma) & (w_fresh, (v_fresh,A)::nil));
-[ | rew_app | rew_app; apply PPermut_last; [permut_simpl | ]]; auto;
+      (Gamma':=Gamma) (G:=G & (w, Gamma) & (w_fresh, (v_fresh,A)::nil)).
 assert (G & (w, Gamma) & (w_fresh, (v_fresh, A) :: nil) ~=~
-  (w_fresh, (v_fresh, A) :: nil) :: emptyEquiv G0) by auto; rewrite H5;
+  (w_fresh, (v_fresh, A) :: nil) :: emptyEquiv G0) by PPermut_simpl; rewrite H7;
 rewrite <- subst_order_irrelevant_bound;
 [eapply HT2; auto | constructor].
+PPermut_simpl; auto.
+PPermut_simpl.
 (* letdia *)
 assert (exists w1, w1 \notin L_w \u free_worlds_LF N) as HF by apply Fresh;
 assert (exists v1, v1 \notin L_t \u free_vars_LF N) as HF2 by apply Fresh;
@@ -1925,7 +1997,7 @@ destruct HF as (w_fresh); destruct HF2 as (v_fresh);
 inversion HT; subst.
 (* letdia #1 *)
 rewrite notin_union in *; destruct H1; destruct H2;
-unfold open_var in *; unfold open_ctx in *;
+unfold open_t in *; unfold open_w in *;
 rewrite subst_t_neutral_free with (v:=v_fresh);
 [ rewrite subst_order_irrelevant_bound |
   apply subst_world_preserv_free_vars]; auto;
@@ -1944,20 +2016,21 @@ assert ( emptyEquiv (G & (w0, nil)) = G & (w0, nil)) by
 [ rewrite <- H6 in HT0 |
   eapply rename_w_preserv_types_outer
     with (G:= (w_fresh, (v_fresh,A)::nil):: G & (w,nil))
-         (Gamma'':=(v_fresh,A)::nil) (Gamma':=nil) (G0:=G)]; auto;
+         (Gamma'':=(v_fresh,A)::nil) (Gamma':=nil) (G0:=G)]; auto.
 rewrite <- subst_order_irrelevant_bound;
 [ eapply HT2; eauto | constructor].
+PPermut_simpl.
 (* letdia #2 *)
 assert (Gamma = nil) by
   (apply emptyEquiv_permut_empty with
-    (G:= (G & (w, Gamma))) (G':=G1) (w:=w); auto; apply Mem_last); subst;
-assert (w <> w0) by eauto;
-assert (w1 <> w) by eauto;
+    (G:= (G & (w, Gamma))) (G':=G1) (w:=w); auto; apply Mem_last); subst.
+assert (w <> w0) by eauto with ok_bg_rew.
+assert (w1 <> w) by eauto with ok_bg_rew.
 rewrite <- H0; rewrite notin_union in *; destruct H1; destruct H2;
-unfold open_var in *; unfold open_ctx in *; destruct (eq_var_dec w1 w0); subst.
+unfold open_t in *; unfold open_w in *; destruct (eq_var_dec w1 w0); subst.
 assert (G0  ~=~ G /\ Gamma0 *=* nil) by
   (apply ok_Bg_impl_ppermut with (w:=w0); eauto);
-destruct H10; apply permut_nil_eq in H11;
+destruct H10; symmetry in H11; apply permut_nil_eq in H11;
 rewrite subst_t_neutral_free with (v:=v_fresh);
 [ eapply subst_t_preserv_types_inner with (A:=A) |
   apply subst_world_preserv_free_vars]; eauto;
@@ -1973,18 +2046,21 @@ rewrite subst_t_neutral_free with (v:=v_fresh);
 apply rename_w_preserv_types_new with
   (G:= (w_fresh, (v_fresh,A)::nil) :: G0 & (w, nil));
 [ rewrite <- subst_order_irrelevant_bound; try constructor; subst |
-  rew_app; eauto];
+  rew_app; eauto].
 rewrite H10; eapply HT2; auto.
+PPermut_simpl.
 assert (Gamma0 = nil) by
   ( apply emptyEquiv_permut_empty with (G:= (G0 & (w1, Gamma0)))
       (G':=G & (w0, nil)) (w:=w1); auto;
     assert (emptyEquiv G = G) by
       (apply emptyEquiv_permut_split_last with (C:=(w, nil)) (H:=G1); auto);
     [ rewrite emptyEquiv_rewrite; simpl | apply Mem_last ]; rewrite H10; auto);
-subst; assert (exists GH, exists GT, G = GH & (w1, nil) ++ GT) by
+subst; assert (exists Gamma'', exists GH, exists GT,
+  Gamma'' *=* nil /\ G = GH & (w1, Gamma'') ++ GT) by
   ( apply PPermut_split_neq with (w:=w0) (G':=G0) (Gamma:=nil);
     [ symmetry | right; intro; subst; elim n]; auto);
-destruct H10 as (GH, H10); destruct H10 as (GT, H10);
+destruct H10 as (Gamma'', (GH, H10)); destruct H10 as (GT, H10).
+destruct H10; symmetry in H10; apply permut_nil_eq in H10; subst.
 rewrite subst_t_neutral_free with (v:=v_fresh);
 [ apply subst_t_preserv_types_outer with (A:=A) (G0 :=GH ++ GT & (w, nil))
           (G := GH ++ GT & (w,nil) & (w1, (v_fresh, A) :: nil))
@@ -1996,7 +2072,8 @@ assert (G0 & (w, nil) ~=~ GH ++ GT & (w,nil) & (w0, nil)) by
       (transitivity ((GH & (w1, nil) ++ GT) & (w0, nil)); rew_app in *; auto);
     assert (G0 ~=~ GH ++ GT & (w0, nil)) by
       (apply PPermut_last_rev_simpl with (a:=(w1,nil)); rew_app in *; auto);
-  rewrite H11; rew_app; auto); rew_app in *; rewrite <- H10;
+  try PPermut_simpl;
+  rewrite H11; rew_app; auto); rew_app in *; rewrite <- H10.
 assert (emptyEquiv G0 = G0) by
 ( assert (G0 ~=~ GH ++ GT & (w0, nil)) by
     ( apply PPermut_last_rev_simpl with (a:=(w, nil));
@@ -2008,7 +2085,7 @@ assert (emptyEquiv G0 = G0) by
   ( apply emptyEquiv_permut_split_last with (C:=(w, nil)) (H:= (w0,nil)::G1);
     simpl; rewrite <- H0; rew_app; symmetry; auto);
   rewrite H11; rewrite H12; rew_app;
-  transitivity (GH ++ (w0, nil) :: (w1, nil)::GT); auto);
+  transitivity (GH ++ (w0, nil) :: (w1, nil)::GT); auto; PPermut_simpl);
 rewrite emptyEquiv_rewrite; simpl; rewrite H11; auto.
 rewrite subst_order_irrelevant_bound;
 [ rewrite <- subst_w_neutral_free with (w0:=w_fresh) | constructor];
@@ -2021,14 +2098,8 @@ rewrite subst_order_irrelevant_bound;
   apply subst_var_preserv_free_worlds]; auto.
 rewrite <- subst_order_irrelevant_bound;
 [eapply HT2; eauto | constructor].
-subst; rew_app;
-transitivity ((w_fresh, (v_fresh, A) :: nil) :: GH ++ GT ++
-  (w, nil) :: (w1, nil) :: nil);
-auto;
-transitivity ((GH ++ GT ++ (w, nil) :: (w1, nil) :: nil) &
-  (w_fresh, (v_fresh, A) :: nil));
-[ | rew_app]; auto.
-rew_app; auto.
+PPermut_simpl.
+PPermut_simpl.
 (* letdia_step *)
 destruct (eq_var_dec w0 w); subst.
 eapply ok_Bg_first_last_neq in Ok_Bg;
